version 6

dimsum/iris/expr2.v
@@ -9,17 +9,15 @@ Set Default Proof Using "Type".
 (** * mod_lang *)
 Structure mod_lang EV Σ := ModLang {
   mexpr : Type;
-  mstate : Type;
   mectx : Type;
   mfill : mectx → mexpr → mexpr;
   mcomp_ectx : mectx → mectx → mectx;
   mtrans :> mod_trans EV;
   mexpr_rel : mtrans.(m_state) → mexpr → Prop;
-  mstate_interp : mtrans.(m_state) → option mstate → iProp Σ;
+  mstate_interp : mtrans.(m_state) → iProp Σ;
   mfill_comp K1 K2 e : mfill K1 (mfill K2 e) = mfill (mcomp_ectx K1 K2) e
 }.
 Global Arguments mexpr {_ _} _.
-Global Arguments mstate {_ _} _.
 Global Arguments mectx {_ _} _.
 Global Arguments mfill {_ _} _.
 Global Arguments mcomp_ectx {_ _} _.
@@ -27,49 +25,78 @@ Global Arguments mtrans {_ _} _.
 Global Arguments mexpr_rel {_ _} _ _ _.
 Global Arguments mstate_interp {_ _} _ _.
 
-(* TODO: better name  *)
-Definition handle_cont {Σ EV} `{!dimsumGS Σ} (m : mod_trans EV) (ts : tgt_src) (Π : option EV → m.(m_state) → iProp Σ)
+Definition switch `{!dimsumGS Σ} {S EV} (Π : option EV → S → iProp Σ)
+  (K : option EV → S → (tgt_src → ∀ m : mod_trans EV, _ → iProp Σ) → iProp Σ) : iProp Σ :=
+  (∀ κ σ, K κ σ (λ ts' m' PΠ', ∀ σ' Π', PΠ' σ' Π' -∗ σ' ≈{ ts', m' }≈> Π') -∗  Π κ σ).
+
+(* Lemma switch_mono `{!dimsumGS Σ} {S EV} (Π : option EV → S → iProp Σ) K1 K2 : *)
+(*   switch Π K1 -∗ *)
+(*   (∀ κ σ P1 P2, K2 κ σ P1 -∗ K1 κ σ P2) -∗ *)
+(*   switch Π K2. *)
+(* Proof. *)
+(*   iIntros "Hs Hmono" (??) "HK2". iApply "Hs". *)
+(*   iApply "Hmono". *)
+
+Definition switch_id `{!dimsumGS Σ} {EV} (ts : tgt_src) (m : mod_trans EV)
+  (Π : option EV → m.(m_state) → iProp Σ)
   (κ : option EV) (σ : m.(m_state)) (C : m.(m_state) → iProp Σ) : iProp Σ :=
-  (∀ σ', C σ' -∗ σ' ≈{ts, m}≈> Π) -∗ Π κ σ.
+  switch Π (λ κs σs POST, ⌜κs = κ⌝ ∗ ⌜σs = σ⌝ ∗
+  POST ts m (λ σ' Πs, ⌜Πs = Π⌝ ∗ C σ'))%I.
 
-Lemma handle_cont_mono {Σ EV} `{!dimsumGS Σ} (m : mod_trans EV) ts Π κ σ C1 C2:
-  handle_cont m ts Π κ σ C1 -∗
-  (∀ σ, C1 σ -∗ C2 σ) -∗
-  handle_cont m ts Π κ σ C2.
-Proof. iIntros "HC Hw Hc". iApply "HC". iIntros (?) "?". iApply "Hc". by iApply "Hw". Qed.
-
-
-Record iModHandler Σ (S EV : Type) := {
-  (* TODO: make this a coercion? *)
-  imodhandle : option EV → S → (S → iProp Σ) → iProp Σ;
-  imodhandle_mono κ σ C C' : imodhandle κ σ C -∗ (∀ σ', C σ' -∗ C' σ') -∗ imodhandle κ σ C';
-}.
-Global Arguments imodhandle {_ _ _}.
-
-Global Instance imodhandle_ne Σ S EV (J : iModHandler Σ S EV) n:
-  Proper ((=) ==> (=) ==> pointwise_relation S (dist n) ==> dist n) (imodhandle J).
+Lemma switch_id_mono `{!dimsumGS Σ} {EV} ts (m : mod_trans EV)
+  (Π : option EV → m.(m_state) → iProp Σ) κ σ C1 C2 :
+  switch_id ts m Π κ σ C1 -∗
+  (∀ σ', C1 σ' -∗ C2 σ') -∗
+  switch_id ts m Π κ σ C2.
 Proof.
-  move => ? κ -> ? σ -> ?? HC.
-  have Heq : (∀ C, imodhandle J κ σ C ⊣⊢ ∃ C', (∀ σ', C' σ' -∗ C σ') ∗ imodhandle J κ σ C').
-  - move => C. apply (anti_symm (⊢)).
-    + iIntros "?". iExists _. iFrame. iIntros (?) "$".
-    + iIntros "(%C'&?&?)". by iApply (imodhandle_mono with "[$]").
-  - rewrite !Heq. by repeat f_equiv.
+  iIntros "Hs Hmono" (??) "[% [% HC2]]". iApply "Hs".
+  iSplit!. iIntros (??) "[% ?]". iApply "HC2". iSplit!.
+  by iApply "Hmono".
 Qed.
 
+(* (* TODO: better name  *) *)
+(* Definition handle_cont {Σ EV} `{!dimsumGS Σ} (m : mod_trans EV) (ts : tgt_src) (Π : option EV → m.(m_state) → iProp Σ) *)
+(*   (κ : option EV) (σ : m.(m_state)) (C : m.(m_state) → iProp Σ) : iProp Σ := *)
+(*   (∀ σ', C σ' -∗ σ' ≈{ts, m}≈> Π) -∗ Π κ σ. *)
 
-Definition subMH {Σ EV} `{!dimsumGS Σ} (m : mod_trans EV) (ts : tgt_src) (J : iModHandler Σ m.(m_state) EV) (Π : option EV → m.(m_state) → iProp Σ) : iProp Σ :=
-  □ (∀ κ σ C, imodhandle J κ σ C -∗ handle_cont m ts Π κ σ C).
+(* Lemma handle_cont_mono {Σ EV} `{!dimsumGS Σ} (m : mod_trans EV) ts Π κ σ C1 C2: *)
+(*   handle_cont m ts Π κ σ C1 -∗ *)
+(*   (∀ σ, C1 σ -∗ C2 σ) -∗ *)
+(*   handle_cont m ts Π κ σ C2. *)
+(* Proof. iIntros "HC Hw Hc". iApply "HC". iIntros (?) "?". iApply "Hc". by iApply "Hw". Qed. *)
 
-Class inMH {Σ EV} `{!dimsumGS Σ} (m : mod_trans EV) (ts : tgt_src) (J : iModHandler Σ m.(m_state) EV) (Π : option EV → m.(m_state) → iProp Σ) :=
-  is_inMH : ⊢ subMH m ts J Π.
 
-Global Hint Mode inMH + + + ! - ! ! : typeclass_instances.
+(* Record iModHandler Σ (S EV : Type) := { *)
+(*   (* TODO: make this a coercion? *) *)
+(*   imodhandle : option EV → S → (S → iProp Σ) → iProp Σ; *)
+(*   imodhandle_mono κ σ C C' : imodhandle κ σ C -∗ (∀ σ', C σ' -∗ C' σ') -∗ imodhandle κ σ C'; *)
+(* }. *)
+(* Global Arguments imodhandle {_ _ _}. *)
 
-Lemma inMH_apply {Σ EV} `{!dimsumGS Σ} {m} (J : iModHandler Σ _ EV) {Π} {ts} (H : inMH m ts J Π) κ σ C :
-  imodhandle J κ σ C -∗
-  handle_cont m ts Π κ σ C.
-Proof. iIntros "?". by iApply (is_inMH (J:=J) (Π:=Π) with "[$]"). Qed.
+(* Global Instance imodhandle_ne Σ S EV (J : iModHandler Σ S EV) n: *)
+(*   Proper ((=) ==> (=) ==> pointwise_relation S (dist n) ==> dist n) (imodhandle J). *)
+(* Proof. *)
+(*   move => ? κ -> ? σ -> ?? HC. *)
+(*   have Heq : (∀ C, imodhandle J κ σ C ⊣⊢ ∃ C', (∀ σ', C' σ' -∗ C σ') ∗ imodhandle J κ σ C'). *)
+(*   - move => C. apply (anti_symm (⊢)). *)
+(*     + iIntros "?". iExists _. iFrame. iIntros (?) "$". *)
+(*     + iIntros "(%C'&?&?)". by iApply (imodhandle_mono with "[$]"). *)
+(*   - rewrite !Heq. by repeat f_equiv. *)
+(* Qed. *)
+
+
+(* Definition subMH {Σ EV} `{!dimsumGS Σ} (m : mod_trans EV) (ts : tgt_src) (J : iModHandler Σ m.(m_state) EV) (Π : option EV → m.(m_state) → iProp Σ) : iProp Σ := *)
+(*   □ (∀ κ σ C, imodhandle J κ σ C -∗ handle_cont m ts Π κ σ C). *)
+
+(* Class inMH {Σ EV} `{!dimsumGS Σ} (m : mod_trans EV) (ts : tgt_src) (J : iModHandler Σ m.(m_state) EV) (Π : option EV → m.(m_state) → iProp Σ) := *)
+(*   is_inMH : ⊢ subMH m ts J Π. *)
+
+(* Global Hint Mode inMH + + + ! - ! ! : typeclass_instances. *)
+
+(* Lemma inMH_apply {Σ EV} `{!dimsumGS Σ} {m} (J : iModHandler Σ _ EV) {Π} {ts} (H : inMH m ts J Π) κ σ C : *)
+(*   imodhandle J κ σ C -∗ *)
+(*   handle_cont m ts Π κ σ C. *)
+(* Proof. iIntros "?". by iApply (is_inMH (J:=J) (Π:=Π) with "[$]"). Qed. *)
 
 (* Lemma subMH_trans Σ S EV (J1 J2 J3 : iModHandler Σ S EV) : *)
 (*   subMH J1 J2 -∗ subMH J2 J3 -∗ subMH J1 J3. *)
@@ -91,40 +118,40 @@ Proof. iIntros "?". by iApply (is_inMH (J:=J) (Π:=Π) with "[$]"). Qed.
 (*   ⊢ subMH J2 (J1 ∪ J2). *)
 (* Proof. iIntros "!>" (???) "HJ". by iRight. Qed. *)
 
-Program Definition nopMH {Σ S EV} : iModHandler Σ S EV := {|
-  imodhandle κ σ C := ⌜κ = None⌝ ∗ C σ;
-|}%I.
-Next Obligation. iIntros (???????) "[-> ?] HC". iSplit; [done|]. by iApply "HC". Qed.
+(* Program Definition nopMH {Σ S EV} : iModHandler Σ S EV := {| *)
+(*   imodhandle κ σ C := ⌜κ = None⌝ ∗ C σ; *)
+(* |}%I. *)
+(* Next Obligation. iIntros (???????) "[-> ?] HC". iSplit; [done|]. by iApply "HC". Qed. *)
 
-Program Definition directMH {Σ EV} {Λ : mod_lang EV Σ} `{!dimsumGS Σ} ts Π : iModHandler Σ (Λ.(m_state)) EV := {|
-  imodhandle κ σ C := (∀ σ', C σ' -∗ σ' ≈{ts, Λ}≈> Π) -∗ Π κ σ;
-|}%I.
-Next Obligation.
-  iIntros (??????????) "HΠ HC". iIntros "Hw". iApply "HΠ". iIntros (?) "?".
-  iApply "Hw". by iApply "HC".
-Qed.
+(* Program Definition directMH {Σ EV} {Λ : mod_lang EV Σ} `{!dimsumGS Σ} ts Π : iModHandler Σ (Λ.(m_state)) EV := {| *)
+(*   imodhandle κ σ C := (∀ σ', C σ' -∗ σ' ≈{ts, Λ}≈> Π) -∗ Π κ σ; *)
+(* |}%I. *)
+(* Next Obligation. *)
+(*   iIntros (??????????) "HΠ HC". iIntros "Hw". iApply "HΠ". iIntros (?) "?". *)
+(*   iApply "Hw". by iApply "HC". *)
+(* Qed. *)
 
 
-Program Definition sim_tgtMH {Σ EV} {m1 : mod_trans EV} `{!dimsumGS Σ}
-  γσ_t γσ_s γκ m1_full Pκ m2 Π
-  : iModHandler Σ (m1.(m_state)) EV := {|
-  imodhandle κ σ C :=
-     (∀ σ', C σ' -∗ σ' ≈{m1}≈>ₜ Π) -∗
-        Pκ κ σ (λ σ_full : m_state m1_full, sim_tgt_constP (m_t:=m1_full) (m_s := m2) γσ_t γσ_s γκ κ σ_full) |}%I.
-Next Obligation.
-  iIntros (???????????????) "HΠ HC". iIntros "Hw". iApply "HΠ". iIntros (?) "?".
-  iApply "Hw". by iApply "HC".
-Qed.
+(* Program Definition sim_tgtMH {Σ EV} {m1 : mod_trans EV} `{!dimsumGS Σ} *)
+(*   γσ_t γσ_s γκ m1_full Pκ m2 Π *)
+(*   : iModHandler Σ (m1.(m_state)) EV := {| *)
+(*   imodhandle κ σ C := *)
+(*      (∀ σ', C σ' -∗ σ' ≈{m1}≈>ₜ Π) -∗ *)
+(*         Pκ κ σ (λ σ_full : m_state m1_full, sim_tgt_constP (m_t:=m1_full) (m_s := m2) γσ_t γσ_s γκ κ σ_full) |}%I. *)
+(* Next Obligation. *)
+(*   iIntros (???????????????) "HΠ HC". iIntros "Hw". iApply "HΠ". iIntros (?) "?". *)
+(*   iApply "Hw". by iApply "HC". *)
+(* Qed. *)
 
-Program Definition switchMH {Σ EV} {m1 : mod_trans EV} `{!dimsumGS Σ} Π Pκ
-  : iModHandler Σ (m1.(m_state)) EV := {|
-  imodhandle κ σ C :=
-     (∀ σ', C σ' -∗ σ' ≈{m1}≈>ₜ Π) -∗
-      Pκ κ σ (λ ts' (m2 : mod_trans EV) σ2 Π2, σ2 ≈{ts', m2}≈> Π2) |}%I.
-Next Obligation.
-  iIntros (??????????)  "HΠ HC". iIntros "Hw". iApply "HΠ". iIntros (?) "?".
-  iApply "Hw". by iApply "HC".
-Qed.
+(* Program Definition switchMH {Σ EV} {m1 : mod_trans EV} `{!dimsumGS Σ} Π Pκ *)
+(*   : iModHandler Σ (m1.(m_state)) EV := {| *)
+(*   imodhandle κ σ C := *)
+(*      (∀ σ', C σ' -∗ σ' ≈{m1}≈>ₜ Π) -∗ *)
+(*       Pκ κ σ (λ ts' (m2 : mod_trans EV) σ2 Π2, σ2 ≈{ts', m2}≈> Π2) |}%I. *)
+(* Next Obligation. *)
+(*   iIntros (??????????)  "HΠ HC". iIntros "Hw". iApply "HΠ". iIntros (?) "?". *)
+(*   iApply "Hw". by iApply "HC". *)
+(* Qed. *)
 
 (** * [sim_gen_expr] *)
 Section sim_gen_expr.
@@ -132,107 +159,76 @@ Section sim_gen_expr.
   Context (ts : tgt_src).
   Implicit Types (e : mexpr Λ).
 
-  (* TODO: Should one be able to change os during the WP? If so, it
-  needs to be added to the postcondition. But it does not seem
-  necessary, I guess one can use a variant of bind for that. *)
-  (* TODO: Change this, to not assert the state interpretation on
-  every step? That seems necessary to be able to go from @ ? None to @
-  ? Some s. However, this would require splitting this definition into
-  two (and break concurrent reasoning, but not sure that we care /
-  that would be the point). *)
   Definition sim_gen_expr_pre (Π : option EV → m_state Λ → iProp Σ)
-    (sim_gen_expr : leibnizO (mexpr Λ) -d> leibnizO (option (mstate Λ)) -d> (leibnizO (mexpr Λ) -d> iPropO Σ) -d> iPropO Σ) :
-    leibnizO (mexpr Λ) -d> leibnizO (option (mstate Λ)) -d> (leibnizO (mexpr Λ) -d> iPropO Σ) -d> iPropO Σ := λ e os Φ,
-    (∀ σ K, ⌜mexpr_rel Λ σ (mfill Λ K e)⌝ -∗ mstate_interp Λ σ os -∗ |={∅}=> ((∃ e', ⌜mexpr_rel Λ σ (mfill Λ K e')⌝ ∗ mstate_interp Λ σ os ∗ Φ e') ∨
-        σ ≈{ ts, Λ }≈> (λ κ σ', handle_cont _ ts Π κ σ' (λ σ'',
-         ∃ e', ⌜mexpr_rel Λ σ'' (mfill Λ K e')⌝ ∗ mstate_interp Λ σ'' os ∗ sim_gen_expr e' os Φ))))%I.
+    (sim_gen_expr : leibnizO (mexpr Λ) -d> (leibnizO (mexpr Λ) -d> iPropO Σ) -d> iPropO Σ) :
+    leibnizO (mexpr Λ) -d> (leibnizO (mexpr Λ) -d> iPropO Σ) -d> iPropO Σ := λ e Φ,
+    (∀ σ K, ⌜mexpr_rel Λ σ (mfill Λ K e)⌝ -∗ mstate_interp Λ σ -∗
+       σ ≈{ ts, Λ }≈> (λ κ σ',
+        (∃ e', ⌜κ = None⌝ ∗ ⌜mexpr_rel Λ σ' (mfill Λ K e')⌝ ∗
+          mstate_interp Λ σ' ∗ Φ e') ∨
+        (switch_id ts Λ Π κ σ' (λ σ'',
+         ∃ e', ⌜mexpr_rel Λ σ'' (mfill Λ K e')⌝ ∗ mstate_interp Λ σ'' ∗ sim_gen_expr e' Φ))))%I.
 
   Global Instance sim_gen_expr_pre_ne Π n:
-    Proper ((dist n ==> dist n ==> dist n ==> dist n) ==> dist n ==> dist n ==> dist n ==> dist n) (sim_gen_expr_pre Π).
+    Proper ((dist n ==> dist n ==> dist n) ==> dist n ==> dist n ==> dist n) (sim_gen_expr_pre Π).
   Proof.
-    move => ?? Hsim ?? -> ?? -> ?? HΦ. rewrite /sim_gen_expr_pre.
+    move => ?? Hsim ?? -> ?? HΦ. rewrite /sim_gen_expr_pre.
     repeat (f_equiv || eapply Hsim || eapply HΦ || reflexivity).
-    move => ?? -> ?? ->. unfold handle_cont.
+    move => ?? -> ?? ->. unfold switch_id, switch.
     repeat (f_equiv || eapply Hsim || eapply HΦ || reflexivity).
   Qed.
 
   Lemma sim_gen_expr_pre_mono J sim1 sim2:
-    ⊢ □ (∀ e os Φ, sim1 e os Φ -∗ sim2 e os Φ)
-    → ∀ e os Φ, sim_gen_expr_pre J sim1 e os Φ -∗ sim_gen_expr_pre J sim2 e os Φ.
+    ⊢ □ (∀ e Φ, sim1 e Φ -∗ sim2 e Φ)
+    → ∀ e Φ, sim_gen_expr_pre J sim1 e Φ -∗ sim_gen_expr_pre J sim2 e Φ.
   Proof.
-    iIntros "#Hinner" (e os Φ) "Hsim". iIntros (???) "?".
-    iMod ("Hsim" with "[//] [$]") as "[?|Hsim]"; [by iLeft; iFrame| iRight; iModIntro].
-    iApply (sim_gen_wand with "Hsim"). iIntros (??) "?". iApply (handle_cont_mono with "[$]").
-    iIntros (?) "(%e'&?&?&?)". iExists _. iFrame. by iApply "Hinner".
+    iIntros "#Hinner" (e Φ) "Hsim". iIntros (???) "?".
+    iSpecialize ("Hsim" with "[//] [$]"). iApply (sim_gen_wand with "Hsim").
+    iIntros (??) "[$|Hsim]". iRight.
+    iApply (switch_id_mono with "Hsim").
+    iIntros (?) "[%e' [% [??]]]". iSplit!; [done|]. iFrame.
+    by iApply "Hinner".
   Qed.
 
   Local Instance sim_gen_expr_pre_monotone J :
-    BiMonoPred (λ sim_gen_expr : prodO (prodO (leibnizO (mexpr Λ)) (leibnizO (option (mstate Λ)))) (leibnizO (mexpr Λ) -d> iPropO Σ) -d> iPropO Σ, uncurry3 (sim_gen_expr_pre J (curry3 sim_gen_expr))).
+    BiMonoPred (λ sim_gen_expr : prodO (leibnizO (mexpr Λ)) (leibnizO (mexpr Λ) -d> iPropO Σ) -d> iPropO Σ, uncurry (sim_gen_expr_pre J (curry sim_gen_expr))).
   Proof.
     constructor.
-    - iIntros (Π Ψ ??) "#Hinner". iIntros ([[??]?]) "Hsim" => /=.
+    - iIntros (Π Ψ ??) "#Hinner". iIntros ([??]) "Hsim" => /=.
       iApply sim_gen_expr_pre_mono; [|done].
-      iIntros "!>" (???) "HΠ". by iApply ("Hinner" $! (_, _, _)).
-    - move => sim_gen Hsim n [[σ1 os1] Φ1] [[σ2 os2] Φ2] /= [[/=??]?].
-      apply sim_gen_expr_pre_ne; eauto. move => ????????? /=. by apply: Hsim.
+      iIntros "!>" (??) "HΠ". by iApply ("Hinner" $! (_, _)).
+    - move => sim_gen Hsim n [σ1 Φ1] [σ2 Φ2] /= [/=??].
+      apply sim_gen_expr_pre_ne; eauto. move => ?????? /=. by apply: Hsim.
   Qed.
 
-  Definition sim_gen_expr J : mexpr Λ → option (mstate Λ) → (mexpr Λ → iProp Σ) → iProp Σ :=
-    curry3 (bi_least_fixpoint (λ sim_gen_expr : prodO (prodO (leibnizO (mexpr Λ)) (leibnizO (option (mstate Λ)))) (leibnizO (mexpr Λ) -d> iPropO Σ) -d> iPropO Σ, uncurry3 (sim_gen_expr_pre J (curry3 sim_gen_expr)))).
+  Definition sim_gen_expr J : mexpr Λ → (mexpr Λ → iProp Σ) → iProp Σ :=
+    curry (bi_least_fixpoint (λ sim_gen_expr : prodO (leibnizO (mexpr Λ)) (leibnizO (mexpr Λ) -d> iPropO Σ) -d> iPropO Σ, uncurry (sim_gen_expr_pre J (curry sim_gen_expr)))).
 
   Global Instance sim_gen_expr_ne J n:
-    Proper ((=) ==> (=) ==> (pointwise_relation _ (dist n)) ==> dist n) (sim_gen_expr J).
-  Proof. move => ?? -> ?? -> ?? HΦ. unfold sim_gen_expr. f_equiv. intros ?. by apply HΦ. Qed.
+    Proper ((=) ==> (pointwise_relation _ (dist n)) ==> dist n) (sim_gen_expr J).
+  Proof. move => ?? -> ?? HΦ. unfold sim_gen_expr. f_equiv. intros ?. by apply HΦ. Qed.
 End sim_gen_expr.
 
 Global Typeclasses Opaque sim_gen_expr.
 
-Notation "'WP{' ts '}' e @ ? os , J {{ Φ } }" := (sim_gen_expr ts J e os Φ%I)
-  (at level 70, Φ at level 200, only parsing) : bi_scope.
-Notation "'WP{' ts '}' e @ s , J {{ Φ } }" := (sim_gen_expr ts J e (Some s) Φ%I)
-  (at level 70, Φ at level 200, only parsing) : bi_scope.
-Notation "'WP{' ts '}' e @ J {{ Φ } }" := (sim_gen_expr ts J e None Φ%I)
+Notation "'WP{' ts '}' e @ J {{ Φ } }" := (sim_gen_expr ts J e Φ%I)
   (at level 70, Φ at level 200, only parsing) : bi_scope.
 
-Notation "'WP{' ts '}' e @ ? os , J {{ e' , Φ } }" := (sim_gen_expr ts J e os (λ e', Φ%I))
-  (at level 70, Φ at level 200,
-    format "'[hv' 'WP{' ts '}'  e  '/' @  ?  os ,  J  {{  '[ ' e' ,  '/' Φ  ']' } } ']'") : bi_scope.
-Notation "'WP{' ts '}' e @ s , J {{ e' , Φ } }" := (sim_gen_expr ts J e (Some s) (λ e', Φ%I))
-  (at level 70, Φ at level 200,
-    format "'[hv' 'WP{' ts '}'  e  '/' @  s ,  J  {{  '[ ' e' ,  '/' Φ  ']' } } ']'") : bi_scope.
-Notation "'WP{' ts '}' e @ J {{ e' , Φ } }" := (sim_gen_expr ts J e None (λ e', Φ%I))
+Notation "'WP{' ts '}' e @ J {{ e' , Φ } }" := (sim_gen_expr ts J e (λ e', Φ%I))
   (at level 70, Φ at level 200,
     format "'[hv' 'WP{' ts '}'  e  '/' @  J  {{  '[ ' e' ,  '/' Φ  ']' } } ']'") : bi_scope.
 
-Notation "'TGT' e @ ? os , J {{ Φ } }" := (sim_gen_expr Tgt J e os Φ%I)
-  (at level 70, Φ at level 200, only parsing) : bi_scope.
-Notation "'TGT' e @ s , J {{ Φ } }" := (sim_gen_expr Tgt J e (Some s) Φ%I)
-  (at level 70, Φ at level 200, only parsing) : bi_scope.
-Notation "'TGT' e @ J {{ Φ } }" := (sim_gen_expr Tgt J e None Φ%I)
+Notation "'TGT' e @ J {{ Φ } }" := (sim_gen_expr Tgt J e Φ%I)
   (at level 70, Φ at level 200, only parsing) : bi_scope.
 
-Notation "'TGT' e @ ? os , J {{ e' , Φ } }" := (sim_gen_expr Tgt J e os (λ e', Φ%I))
-  (at level 70, Φ at level 200,
-    format "'[hv' 'TGT'  e  '/' @  ?  os ,  J  {{  '[ ' e' ,  '/' Φ  ']' } } ']'") : bi_scope.
-Notation "'TGT' e @ s , J {{ e' , Φ } }" := (sim_gen_expr Tgt J e (Some s) (λ e', Φ%I))
-  (at level 70, Φ at level 200,
-    format "'[hv' 'TGT'  e  '/' @  s ,  J  {{  '[ ' e' ,  '/' Φ  ']' } } ']'") : bi_scope.
-Notation "'TGT' e @ J {{ e' , Φ } }" := (sim_gen_expr Tgt J e None (λ e', Φ%I))
+Notation "'TGT' e @ J {{ e' , Φ } }" := (sim_gen_expr Tgt J e (λ e', Φ%I))
   (at level 70, Φ at level 200,
     format "'[hv' 'TGT'  e  '/' @  J  {{  '[ ' e' ,  '/' Φ  ']' } } ']'") : bi_scope.
 
-Notation "'SRC' e @ ? os , J {{ Φ } }" := (sim_gen_expr Src J e os  Φ%I)
-  (at level 70, Φ at level 200, only parsing) : bi_scope.
-Notation "'SRC' e @ s , J {{ Φ } }" := (sim_gen_expr Src J e (Some s) Φ%I)
-  (at level 70, Φ at level 200, only parsing) : bi_scope.
-Notation "'SRC' e @ J {{ Φ } }" := (sim_gen_expr Src J e None Φ%I)
+Notation "'SRC' e @ J {{ Φ } }" := (sim_gen_expr Src J e Φ%I)
   (at level 70, Φ at level 200, only parsing) : bi_scope.
 
-Notation "'SRC' e @ ? os , J {{ e' , Φ } }" := (sim_gen_expr Src J e os (λ e', Φ%I)) (at level 70, Φ at level 200,
-  format "'[hv' 'SRC'  e  '/' @  ?  os , J  {{  '[ ' e' ,  '/' Φ  ']' } } ']'") : bi_scope.
-Notation "'SRC' e @ s , J {{ e' , Φ } }" := (sim_gen_expr Src J e (Some s) (λ e', Φ%I)) (at level 70, Φ at level 200,
-  format "'[hv' 'SRC'  e  '/' @  s ,  J  {{  '[ ' e' ,  '/' Φ  ']' } } ']'") : bi_scope.
-Notation "'SRC' e @ J {{ e' , Φ } }" := (sim_gen_expr Src J e None (λ e', Φ%I)) (at level 70, Φ at level 200,
+Notation "'SRC' e @ J {{ e' , Φ } }" := (sim_gen_expr Src J e (λ e', Φ%I)) (at level 70, Φ at level 200,
   format "'[hv' 'SRC'  e  '/' @  J  {{  '[ ' e' ,  '/' Φ  ']' } } ']'") : bi_scope.
 
 Section sim_gen_expr.
@@ -241,97 +237,106 @@ Section sim_gen_expr.
   Implicit Types (e : mexpr Λ).
 
   Local Existing Instance sim_gen_expr_pre_monotone.
-  Lemma sim_gen_expr_unfold e Π os Φ:
-    WP{ts} e @ ? os, Π {{ Φ }} ⊣⊢ sim_gen_expr_pre ts Π (sim_gen_expr ts Π) e os Φ.
-  Proof. rewrite /sim_gen_expr /curry3. apply: least_fixpoint_unfold. Qed.
+  Lemma sim_gen_expr_unfold e Π Φ:
+    WP{ts} e @ Π {{ Φ }} ⊣⊢ sim_gen_expr_pre ts Π (sim_gen_expr ts Π) e Φ.
+  Proof. rewrite /sim_gen_expr /curry. apply: least_fixpoint_unfold. Qed.
 
-  Lemma sim_gen_expr_strong_ind Π (R: leibnizO (mexpr Λ) -d> leibnizO (option (mstate Λ)) -d> (leibnizO (mexpr Λ) -d> iPropO Σ) -d> iPropO Σ):
-    NonExpansive3 R →
-    ⊢ (□ ∀ e os Φ, sim_gen_expr_pre ts Π (λ e os Φ, R e os Φ ∧ WP{ts} e @ ? os, Π {{Φ}}) e os Φ -∗ R e os Φ)
-      -∗ ∀ e os Φ, WP{ts} e @ ? os, Π {{Φ}} -∗ R e os Φ.
+  Lemma sim_gen_expr_strong_ind Π (R: leibnizO (mexpr Λ) -d> (leibnizO (mexpr Λ) -d> iPropO Σ) -d> iPropO Σ):
+    NonExpansive2 R →
+    ⊢ (□ ∀ e Φ, sim_gen_expr_pre ts Π (λ e Φ, R e Φ ∧ WP{ts} e @ Π {{Φ}}) e Φ -∗ R e Φ)
+      -∗ ∀ e Φ, WP{ts} e @ Π {{Φ}} -∗ R e Φ.
   Proof.
-    iIntros (Hne) "#HPre". iIntros (e os Φ) "Hsim".
-    rewrite {2}/sim_gen_expr {1}/curry3.
-    iApply (least_fixpoint_ind _ (uncurry3 R) with "[] Hsim").
-    iIntros "!>" ([[??]?]) "Hsim" => /=. by iApply "HPre".
+    iIntros (Hne) "#HPre". iIntros (e Φ) "Hsim".
+    rewrite {2}/sim_gen_expr {1}/curry.
+    iApply (least_fixpoint_ind _ (uncurry R) with "[] Hsim").
+    iIntros "!>" ([??]) "Hsim" => /=. by iApply "HPre".
   Qed.
 
-  Lemma sim_gen_expr_ind Π (R: leibnizO (mexpr Λ) -d> leibnizO (option (mstate Λ)) -d> (leibnizO (mexpr Λ) -d> iPropO Σ) -d> iPropO Σ) :
-    NonExpansive3 R →
-    ⊢ (□ ∀ e os Φ, sim_gen_expr_pre ts Π R e os Φ -∗ R e os Φ)
-      -∗ ∀ e os Φ, WP{ts} e @ ? os, Π {{ Φ }} -∗ R e os Φ.
+  Lemma sim_gen_expr_ind Π (R: leibnizO (mexpr Λ) -d> (leibnizO (mexpr Λ) -d> iPropO Σ) -d> iPropO Σ) :
+    NonExpansive2 R →
+    ⊢ (□ ∀ e Φ, sim_gen_expr_pre ts Π R e Φ -∗ R e Φ)
+      -∗ ∀ e Φ, WP{ts} e @ Π {{ Φ }} -∗ R e Φ.
   Proof.
-    iIntros (Hne) "#HPre". iApply sim_gen_expr_strong_ind. iIntros "!>" (e os Φ) "Hsim".
+    iIntros (Hne) "#HPre". iApply sim_gen_expr_strong_ind.
+    iIntros "!>" (e Φ) "Hsim".
     iApply "HPre". iApply (sim_gen_expr_pre_mono with "[] Hsim").
-    iIntros "!>" (???) "[? _]". by iFrame.
+    iIntros "!>" (??) "[? _]". by iFrame.
   Qed.
 
-  Lemma sim_gen_expr_wand e os Π Φ Ψ :
-    WP{ts} e @ ? os, Π {{ Ψ }} -∗
+  Lemma sim_gen_expr_wand e Π Φ Ψ :
+    WP{ts} e @ Π {{ Ψ }} -∗
     (∀ e', Ψ e' -∗ Φ e') -∗
-    WP{ts} e @ ? os, Π {{ Φ }}.
+    WP{ts} e @ Π {{ Φ }}.
   Proof.
     iIntros "HWP Hwand".
-    pose (F := (λ e os Ψ, ∀ Φ,
+    pose (F := (λ e Ψ, ∀ Φ,
         (∀ e', Ψ e' -∗ Φ e') -∗
-         WP{ts} e @ ? os, Π {{Φ}})%I).
-    iAssert (∀ Ψ, WP{ts} e @ ? os, Π {{Ψ}} -∗ F e os Ψ)%I as "Hgen"; last first.
+         WP{ts} e @ Π {{Φ}})%I).
+    iAssert (∀ Ψ, WP{ts} e @ Π {{Ψ}} -∗ F e Ψ)%I as "Hgen"; last first.
     { iApply ("Hgen" with "HWP"). iIntros (?) "?". by iApply "Hwand". }
     iIntros (?) "Hsim".
     iApply (sim_gen_expr_ind with "[] Hsim"). { solve_proper. }
-    iIntros "!>" (???) "Hsim". iIntros (?) "Hc".
+    iIntros "!>" (??) "Hsim". iIntros (?) "Hc".
     rewrite sim_gen_expr_unfold. iIntros (???) "?".
-    iMod ("Hsim" with "[//] [$]") as "[[% [% [? HΦ]]]|Hsim]"; iModIntro.
-    - iLeft. iExists _. iSplit; [done|]. iFrame. by iApply "Hc".
-    - iRight. iApply (sim_gen_wand with "Hsim"). iIntros (? ?) "Hsim /=".
-      iApply (handle_cont_mono with "Hsim"). iIntros (?) "(%e'&?&?&Hsim)". iExists _. iFrame.
-      by iApply "Hsim".
+    iSpecialize ("Hsim" with "[//] [$]").
+    iApply (sim_gen_wand with "Hsim").
+    iIntros (? ?) "[[% [% [% [? HΦ]]]]|Hsim] /=".
+    - iLeft. iExists _. iSplit!; [done|]. iFrame. by iApply "Hc".
+    - iRight. iApply (switch_id_mono with "Hsim"). iIntros (?) "[% [% [? Hsim]]] /=".
+      iFrame. iSplit!; [done|]. by iApply "Hsim".
   Qed.
 
-  Lemma sim_gen_expr_bind K e os Π Φ :
-    WP{ts} e @ ? os, Π {{ e', WP{ts} mfill Λ K e' @ ? os , Π {{Φ}} }} -∗
-    WP{ts} mfill Λ K e @ ? os, Π {{ Φ }}.
+  Lemma sim_gen_expr_bind K e Π Φ :
+    WP{ts} e @ Π {{ e', WP{ts} mfill Λ K e' @ Π {{Φ}} }} -∗
+    WP{ts} mfill Λ K e @ Π {{ Φ }}.
   Proof.
     iIntros "HWP".
-    pose (F := (λ e os' Ψ, ∀ Φ, ⌜os' = os⌝ -∗
-        (∀ e', Ψ e' -∗ WP{ts} mfill Λ K e' @ ? os, Π {{Φ}}) -∗
-         WP{ts} mfill Λ K e @ ? os , Π {{Φ}})%I).
-    iAssert (∀ Ψ, WP{ts} e @ ? os , Π {{Ψ}} -∗ F e os Ψ)%I as "Hgen"; last first.
-    { iApply ("Hgen" with "HWP [//]"). iIntros (?) "?". done. }
+    pose (F := (λ e Ψ, ∀ Φ,
+        (∀ e', Ψ e' -∗ WP{ts} mfill Λ K e' @ Π {{Φ}}) -∗
+         WP{ts} mfill Λ K e @ Π {{Φ}})%I).
+    iAssert (∀ Ψ, WP{ts} e @ Π {{Ψ}} -∗ F e Ψ)%I as "Hgen"; last first.
+    { iApply ("Hgen" with "HWP"). iIntros (?) "?". done. }
     iIntros (?) "Hsim".
     iApply (sim_gen_expr_ind with "[] Hsim"). { solve_proper. }
-    iIntros "!>" (???) "Hsim". iIntros (? ?) "Hc". subst.
+    iIntros "!>" (??) "Hsim". iIntros (?) "Hc".
     rewrite sim_gen_expr_unfold. iIntros (?? Hf) "?". rewrite mfill_comp in Hf.
-    iMod ("Hsim" with "[//] [$]") as "[[% [% [? HΦ]]]|Hsim]".
-    - iSpecialize ("Hc" with "[$]"). rewrite sim_gen_expr_unfold.
+    iApply sim_gen_bind.
+    iSpecialize ("Hsim" with "[//] [$]").
+    iApply (sim_gen_wand with "Hsim").
+    iIntros (? ?) "[[% [% [% [? HΦ]]]]|Hsim] /=".
+    - iRight. iSpecialize ("Hc" with "[$]"). rewrite sim_gen_expr_unfold.
       iDestruct ("Hc" with "[] [$]") as "?". { by rewrite mfill_comp. }
-      done.
-    - iModIntro. iRight. iApply (sim_gen_wand with "Hsim"). iIntros (??) "Hsim /=".
-      iApply (handle_cont_mono with "Hsim"). iIntros (?) "(%e'&?&?&Hsim)". rewrite -mfill_comp.
-      iExists _. iFrame. by iApply "Hsim".
+      iSplit!.
+    - iLeft. iRight. iApply (switch_id_mono with "Hsim").
+      iIntros (?) "[% [%Hf' [? Hsim]]] /=". rewrite -mfill_comp in Hf'.
+      iFrame. iSplit!; [done|]. by iApply "Hsim".
   Qed.
 
-  Lemma sim_gen_expr_bind0 e os Π Φ :
-    WP{ts} e @ ? os, Π {{ e', WP{ts} e' @ ? os , Π {{Φ}} }} -∗
-    WP{ts} e @ ? os, Π {{ Φ }}.
+  (* TODO: derive this lemma from the previous by requiring an empty context? *)
+  Lemma sim_gen_expr_bind0 e Π Φ :
+    WP{ts} e @ Π {{ e', WP{ts} e' @ Π {{Φ}} }} -∗
+    WP{ts} e @ Π {{ Φ }}.
   Proof.
     iIntros "HWP".
-    pose (F := (λ e os' Ψ, ∀ Φ, ⌜os' = os⌝ -∗
-        (∀ e', Ψ e' -∗ WP{ts} e' @ ? os, Π {{Φ}}) -∗
-         WP{ts} e @ ? os , Π {{Φ}})%I).
-    iAssert (∀ Ψ, WP{ts} e @ ? os , Π {{Ψ}} -∗ F e os Ψ)%I as "Hgen"; last first.
-    { iApply ("Hgen" with "HWP [//]"). iIntros (?) "?". done. }
+    pose (F := (λ e Ψ, ∀ Φ,
+        (∀ e', Ψ e' -∗ WP{ts} e' @ Π {{Φ}}) -∗
+         WP{ts} e @ Π {{Φ}})%I).
+    iAssert (∀ Ψ, WP{ts} e @ Π {{Ψ}} -∗ F e Ψ)%I as "Hgen"; last first.
+    { iApply ("Hgen" with "HWP"). iIntros (?) "?". done. }
     iIntros (?) "Hsim".
     iApply (sim_gen_expr_ind with "[] Hsim"). { solve_proper. }
-    iIntros "!>" (???) "Hsim". iIntros (? ?) "Hc". subst.
+    iIntros "!>" (??) "Hsim". iIntros (?) "Hc".
     rewrite sim_gen_expr_unfold. iIntros (?? Hf) "?".
-    iMod ("Hsim" with "[//] [$]") as "[[% [% [? HΦ]]]|Hsim]".
-    - iSpecialize ("Hc" with "[$]"). rewrite sim_gen_expr_unfold.
-      iDestruct ("Hc" with "[] [$]") as "?". { done. }
-      done.
-    - iModIntro. iRight. iApply (sim_gen_wand with "Hsim"). iIntros (??) "Hsim /=".
-      iApply (handle_cont_mono with "Hsim"). iIntros (?) "(%e'&?&?&Hsim)".
-      iExists _. iFrame. by iApply "Hsim".
+    iApply sim_gen_bind.
+    iSpecialize ("Hsim" with "[//] [$]").
+    iApply (sim_gen_wand with "Hsim").
+    iIntros (? ?) "[[% [% [% [? HΦ]]]]|Hsim] /=".
+    - iRight. iSpecialize ("Hc" with "[$]"). rewrite sim_gen_expr_unfold.
+      iDestruct ("Hc" with "[//] [$]") as "?".
+      iSplit!.
+    - iLeft. iRight. iApply (switch_id_mono with "Hsim").
+      iIntros (?) "[% [%Hf' [? Hsim]]] /=".
+      iFrame. iSplit!; [done|]. by iApply "Hsim".
   Qed.
 
   (*
@@ -356,68 +361,91 @@ Section sim_gen_expr.
   Qed.
    *)
 
-  Definition direct_post (K : mectx Λ) (os : option (mstate Λ)) (Π : option EV → m_state Λ → iProp Σ) (e : mexpr Λ) : iProp Σ :=
-    ∀ σ', ⌜mexpr_rel Λ σ' (mfill Λ K e)⌝ -∗ mstate_interp Λ σ' os -∗ σ' ≈{ts, Λ}≈> Π.
+  Definition sim_post (K : mectx Λ) (Π : option EV → m_state Λ → iProp Σ) (e : mexpr Λ) : iProp Σ :=
+    ∀ σ', ⌜mexpr_rel Λ σ' (mfill Λ K e)⌝ -∗ mstate_interp Λ σ' -∗ σ' ≈{ts, Λ}≈> Π.
 
   (* Be careful when choosing Π when applying this rule, it must never change! *)
-  Lemma sim_gen_expr_intro K e os Π σ :
+  Lemma sim_gen_expr_intro K e Π σ :
     mexpr_rel Λ σ (mfill Λ K e) →
-    mstate_interp Λ σ os -∗
-    WP{ts} e @ ? os, Π {{ direct_post K os Π }} -∗
+    mstate_interp Λ σ -∗
+    WP{ts} e @ Π {{ sim_post K Π }} -∗
     σ ≈{ts, Λ}≈> Π.
   Proof.
     iIntros (?) "Hσ Hsim".
-    pose (F := (λ e os' Ψ, ∀ σ, ⌜mexpr_rel Λ σ (mfill Λ K e)⌝ -∗ ⌜os' = os⌝ -∗ mstate_interp Λ σ os -∗
-       (∀ e', Ψ e' -∗ direct_post K os Π e') -∗
+    pose (F := (λ e Ψ, ∀ σ, ⌜mexpr_rel Λ σ (mfill Λ K e)⌝ -∗ mstate_interp Λ σ -∗
+       (∀ e', Ψ e' -∗ sim_post K Π e') -∗
        σ ≈{ ts, Λ }≈> Π)%I).
-    iAssert (∀ e Φ, WP{ts} e @ ? os, Π {{Φ}} -∗ F e os Φ)%I as "Hgen"; last first.
-    { iApply ("Hgen" with "Hsim [//] [//] Hσ"). iIntros (?) "$". }
+    iAssert (∀ e Φ, WP{ts} e @ Π {{Φ}} -∗ F e Φ)%I as "Hgen"; last first.
+    { iApply ("Hgen" with "Hsim [//] Hσ"). iIntros (?) "$". }
     iIntros (??) "Hsim".
     iApply (sim_gen_expr_ind with "[] Hsim"). { solve_proper. }
-    iIntros "!>" (???) "Hsim". iIntros (???) "Hσ HΦ". subst.
-    iApply fupd_sim_gen.
-    iDestruct ("Hsim" with "[//] Hσ") as ">[[% [% [Hσ Hsim]]]|Hsim]"; iModIntro.
-    { by iApply ("HΦ" with "Hsim [//] Hσ"). }
-    iApply (sim_gen_wand with "Hsim"). iIntros (κ σ1) "Hhandler".
-    iApply "Hhandler". iIntros (?) "[%e'[%[? HF]]]". iApply ("HF" with "[//] [//] [$] [$]").
-  Qed.
+    iIntros "!>" (??) "Hsim". iIntros (??) "Hσ HΦ".
+    iSpecialize ("Hsim" with "[//] Hσ").
+    iApply sim_gen_bind. iApply (sim_gen_wand with "Hsim").
+    iIntros (??) "[[% [% [% [??]]]]|Hsim]".
+    - iRight. iSplit!. iApply ("HΦ" with "[$] [//] [$]").
+    - iLeft. iApply "Hsim". iSplit!. iIntros (??) "[% [% [% [? HF]]]]". subst.
+      iApply ("HF" with "[//] [$] [$]").
+Qed.
 
-  Lemma sim_gen_expr_ctx e Π os Φ :
-    (ord_later_ctx -∗ WP{ts} e @ ? os, Π {{ Φ }}) -∗
-    WP{ts} e @ ? os, Π {{ Φ }}.
-  Proof. Admitted.
-
-  Lemma fupd_sim_gen_expr e os Π Φ :
-    (|={∅}=> WP{ts} e @ ? os, Π {{ Φ }}) -∗
-    WP{ts} e @ ? os, Π {{ Φ }}.
-  Proof. iIntros "Hsim". rewrite sim_gen_expr_unfold. by iMod "Hsim". Qed.
-
-  Lemma sim_gen_expr_end e Π os Φ :
-    Φ e -∗ WP{ts} e @ ? os , Π {{ Φ }}.
+  Lemma sim_gen_expr_ctx e Π Φ :
+    (ord_later_ctx -∗ WP{ts} e @ Π {{ Φ }}) -∗
+    WP{ts} e @ Π {{ Φ }}.
   Proof.
-    iIntros "HΦ". rewrite sim_gen_expr_unfold. iIntros (??) "HF ?".
-    iModIntro. iLeft. iExists _. iSplit; [done|]. iFrame.
+    iIntros "Hsim". rewrite sim_gen_expr_unfold. iIntros (???) "?".
+    iApply sim_gen_ctx. iIntros "?". iApply ("Hsim" with "[$] [//] [$]").
   Qed.
 
-  Lemma sim_gen_expr_steps e os Π Φ :
-    (∀ σ K, ⌜mexpr_rel Λ σ (mfill Λ K e)⌝ -∗ mstate_interp Λ σ os -∗
-          σ ≈{ ts, Λ }≈> (λ κ σ', handle_cont _ ts Π κ σ' (λ σ'',
-             ∃ e', ⌜mexpr_rel Λ σ'' (mfill Λ K e')⌝ ∗ mstate_interp Λ σ'' os ∗ WP{ts} e' @ ? os , Π {{Φ}}))) -∗
-    WP{ts} e @ ? os , Π {{ Φ }}.
+  Lemma fupd_sim_gen_expr e Π Φ :
+    (|={∅}=> WP{ts} e @ Π {{ Φ }}) -∗
+    WP{ts} e @ Π {{ Φ }}.
   Proof.
-    iIntros "HΦ". rewrite sim_gen_expr_unfold. iIntros (???) "? !>". iRight.
-    iApply (sim_gen_wand with "[-]"). { by iApply "HΦ". } by iIntros (??) "?".
+    iIntros "Hsim". rewrite sim_gen_expr_unfold.
+    iIntros (???) "?". iApply fupd_sim_gen.
+    iMod "Hsim". by iApply "Hsim".
   Qed.
 
-  Lemma sim_gen_expr_None e os Π Φ :
-    (∀ σ K, ⌜mexpr_rel Λ σ (mfill Λ K e)⌝ -∗ mstate_interp Λ σ os -∗
-          handle_cont _ ts Π None σ (λ σ'',
-             ∃ e', ⌜mexpr_rel Λ σ'' (mfill Λ K e')⌝ ∗ mstate_interp Λ σ'' os ∗ WP{ts} e' @ ? os , Π {{Φ}})) -∗
-    WP{ts} e @ ? os , Π {{ Φ }}.
+  Lemma sim_gen_expr_stop e Π Φ :
+    Φ e -∗ WP{ts} e @ Π {{ Φ }}.
   Proof.
-    iIntros "HΦ". iApply sim_gen_expr_steps. iIntros (???) "?".
-    iApply sim_gen_stop. by iApply "HΦ".
+    iIntros "HΦ". rewrite sim_gen_expr_unfold. iIntros (???) "HF".
+    iApply sim_gen_stop. iLeft. iSplit!; [done|]. iFrame.
   Qed.
+
+  Lemma sim_gen_expr_steps_None e Π Φ :
+    (∀ σ K, ⌜mexpr_rel Λ σ (mfill Λ K e)⌝ -∗ mstate_interp Λ σ -∗
+          σ ≈{ ts, Λ }≈> (λ κ σ', ∃ e',
+           ⌜κ = None⌝ ∗ ⌜mexpr_rel Λ σ' (mfill Λ K e')⌝ ∗
+           mstate_interp Λ σ' ∗ WP{ts} e' @ Π {{Φ}})) -∗
+    WP{ts} e @ Π {{ Φ }}.
+  Proof.
+    iIntros "HΦ". rewrite sim_gen_expr_unfold. iIntros (???) "?".
+    iApply sim_gen_bind.
+    iApply (sim_gen_wand with "[-]"). { by iApply "HΦ". }
+    iIntros (??) "[% [% [% [? Hsim]]]]". iRight. iSplit!.
+    rewrite sim_gen_expr_unfold. by iApply "Hsim".
+  Qed.
+
+  Lemma sim_gen_expr_steps e Π Φ :
+    (∀ σ K, ⌜mexpr_rel Λ σ (mfill Λ K e)⌝ -∗ mstate_interp Λ σ -∗
+          σ ≈{ ts, Λ }≈> (λ κ σ', switch_id ts Λ Π κ σ' (λ σ'',
+             ∃ e', ⌜mexpr_rel Λ σ'' (mfill Λ K e')⌝ ∗ mstate_interp Λ σ'' ∗ WP{ts} e' @ Π {{Φ}}))) -∗
+    WP{ts} e @ Π {{ Φ }}.
+  Proof.
+    iIntros "HΦ". rewrite sim_gen_expr_unfold. iIntros (???) "?".
+    iApply (sim_gen_wand with "[-]"). { by iApply "HΦ". }
+    iIntros (??) "?". iRight. done.
+  Qed.
+
+  (* Lemma sim_gen_expr_None e os Π Φ : *)
+  (*   (∀ σ K, ⌜mexpr_rel Λ σ (mfill Λ K e)⌝ -∗ mstate_interp Λ σ os -∗ *)
+  (*         handle_cont _ ts Π None σ (λ σ'', *)
+  (*            ∃ e', ⌜mexpr_rel Λ σ'' (mfill Λ K e')⌝ ∗ mstate_interp Λ σ'' os ∗ WP{ts} e' @ ? os , Π {{Φ}})) -∗ *)
+  (*   WP{ts} e @ ? os , Π {{ Φ }}. *)
+  (* Proof. *)
+  (*   iIntros "HΦ". iApply sim_gen_expr_steps. iIntros (???) "?". *)
+  (*   iApply sim_gen_stop. by iApply "HΦ". *)
+  (* Qed. *)
 End sim_gen_expr.
 
 (*
