dimsum_examples/iris/rec2.v
@@ -13,8 +13,7 @@ Notation "'let*' x , .. , z := t 'in' f" :=
     (at level 200, x closed binder, z closed binder) : stdpp_scope.
 Notation "'let*' := t 'in' f" := (t f) (only parsing, at level 200) : stdpp_scope.
 
-(* TODO: Rename Π to position or event handler and add Type of parameters and nop requirement and parametrize by ts? *)
-
+(* TODO: Rename Π to position or event handler and add Type of parameters and nop requirement and parametrize by ts? -> No *)
 
 (* TODO: upstream *)
 Global Instance spec_inhabited EV S R : Inhabited (spec EV S R) := populate TUb.
@@ -25,12 +24,11 @@ Global Instance rec_state_inhabited : Inhabited rec_state := populate (Rec inhab
 Program Canonical Structure rec_mod_lang {Σ} `{!recGS Σ} := {|
   mexpr := expr;
   mectx := list expr_ectx;
-  mstate := heap_state;
   mfill := expr_fill;
   mcomp_ectx := flip app;
   mtrans := rec_trans;
   mexpr_rel σ e := st_expr σ = e;
-  mstate_interp := rec_state_interp;
+  mstate_interp σ := rec_state_interp σ None;
 |}.
 Next Obligation. move => ?????/=. by rewrite expr_fill_app. Qed.
 
@@ -83,7 +81,7 @@ Section lifting.
       rec_fn_auth fns -∗
       rec_mapsto_auth (h_heap h) -∗
       rec_alloc_auth (dom (h_heap h)) -∗
-      ▷ₒ handle_cont rec_trans Tgt Π (Some (Outgoing, ERReturn v h)) (Rec (expr_fill K (Waiting b)) h fns) (λ σ,
+      ▷ₒ switch_id Tgt rec_trans Π (Some (Outgoing, ERReturn v h)) (Rec (expr_fill K (Waiting b)) h fns) (λ σ,
          ∃ e', ⌜st_expr σ = expr_fill K e'⌝ ∗ ⌜st_fns σ = fns⌝ ∗
          rec_mapsto_auth (h_heap (st_heap σ)) ∗
          rec_alloc_auth (dom (h_heap (st_heap σ))) ∗ Φ e')) -∗
@@ -97,18 +95,19 @@ Section lifting.
     { done. }
     move => [? [Hstep ?]]. inv Hstep.
     iSpecialize ("HΦ" $! _ with "[$] [$] [$]"). iModIntro. iSplit!.
-    do 2 iModIntro. iApply (handle_cont_mono with "HΦ"). iIntros (?) "[% [% [% [?[??]]]]]".
-    iSplit!; [done|]. iFrame. subst. iFrame "#". by iApply sim_gen_expr_end.
+    do 2 iModIntro. iApply (switch_id_mono with "HΦ").
+    iIntros (?) "[% [% [% [?[??]]]]]".
+    iSplit!; [done|]. iFrame. subst. iFrame "#". by iApply sim_gen_expr_stop.
   Qed.
 
-  (* TODO: can we somehow get rid of the nopMH requirement? *)
-  Lemma sim_tgt_rec_Call_internal f fn es Π Φ vs `{!AsVals es vs None} `{!inMH _ Tgt nopMH Π} :
+  Lemma sim_tgt_rec_Call_internal f fn es Π Φ vs `{!AsVals es vs None} :
     length vs = length (fd_args fn) →
     f ↪ Some fn -∗
     (▷ₒ TGT AllocA fn.(fd_vars) (subst_static f (fd_static_vars fn) (subst_l (fd_args fn) vs (fd_body fn))) @ Π {{ Φ }}) -∗
     TGT Call (Val (ValFn f)) es @ Π {{ Φ }}.
   Proof.
-    destruct AsVals0. iIntros (?) "Hfn HΦ". iApply (sim_gen_expr_steps with "[-]") => /=.
+    destruct AsVals0. iIntros (?) "Hfn HΦ".
+    iApply (sim_gen_expr_steps_None with "[-]") => /=.
     iIntros ([e h0 fns0] ??) "[#Hfns [Hh Ha]]". simplify_eq/=.
     iApply (sim_tgt_step_end with "[-]"). iIntros (?? Hp). simplify_eq/=.
     iDestruct (rec_fn_lookup with "[$] [$]") as %?.
@@ -118,7 +117,7 @@ Section lifting.
       move => /= ??? e' [_ Heq]. by apply: list_expr_val_inv. }
     { done. }
     move => [? [Hstep ?]]. inv Hstep.
-    iModIntro. iSplit!. do 2 iModIntro. iApply (inMH_apply nopMH with "[-]"). iSplit!. iFrame "∗#".
+    iModIntro. iSplit!. do 2 iModIntro. iSplit!. iFrame "∗#".
   Qed.
 
   Lemma sim_tgt_rec_Call_external f es Π Φ vs `{!AsVals es vs None} :
@@ -127,7 +126,7 @@ Section lifting.
       rec_fn_auth fns -∗
       rec_mapsto_auth (h_heap h) -∗
       rec_alloc_auth (dom (h_heap h)) -∗
-      ▷ₒ handle_cont rec_trans Tgt Π (Some (Outgoing, ERCall f vs h))
+      ▷ₒ switch_id Tgt rec_trans Π (Some (Outgoing, ERCall f vs h))
         (Rec (expr_fill K (Waiting true)) h fns) (λ σ,
           ∃ e', ⌜st_expr σ = expr_fill K e'⌝ ∗ ⌜st_fns σ = fns⌝ ∗
            rec_mapsto_auth (h_heap (st_heap σ)) ∗
@@ -145,32 +144,32 @@ Section lifting.
     { done. }
     move => [? [Hstep ?]]. inv Hstep.
     iSpecialize ("HΦ" $! _ with "[$] [$] [$]"). iModIntro. iSplit!. do 2 iModIntro.
-    iApply (handle_cont_mono with "HΦ"). iIntros (?) "[% [% [% [?[??]]]]]".
-    iSplit!; [done|]. iFrame. subst. iFrame "#". by iApply sim_gen_expr_end.
+    iApply (switch_id_mono with "HΦ"). iIntros (?) "[% [% [% [?[??]]]]]".
+    iSplit!; [done|]. iFrame. subst. iFrame "#". by iApply sim_gen_expr_stop.
   Qed.
 
-  Lemma sim_tgt_rec_BinOp Π Φ v1 v2 v3 op `{!inMH _ Tgt nopMH Π} :
+  Lemma sim_tgt_rec_BinOp Π Φ v1 v2 v3 op :
     eval_binop op v1 v2 = Some v3 →
     (▷ₒ Φ (Val v3)) -∗
     TGT BinOp (Val v1) op (Val v2) @ Π {{ Φ }}.
   Proof.
-    iIntros (Hop) "HΦ". iApply (sim_gen_expr_steps with "[-]") => /=.
+    iIntros (Hop) "HΦ". iApply (sim_gen_expr_steps_None with "[-]") => /=.
     iIntros ([e h0 fns0] ??) "[#Hfns [Hh Ha]]". simplify_eq/=.
     iApply (sim_tgt_step_end with "[-]"). iIntros (?? Hp). simplify_eq/=.
     exploit prim_step_inv_head; [done|..].
     { apply sub_redexes_are_values_item; case; naive_solver. }
     { done. }
     move => [? [Hstep ?]]. inv Hstep.
-    iModIntro. iSplit!. do 2 iModIntro. iApply (inMH_apply nopMH with "[-]"). iSplit!. iFrame "∗#".
-    by iApply sim_gen_expr_end.
+    iModIntro. iSplit!. do 2 iModIntro. iSplit!. iFrame "∗#".
+    by iApply sim_gen_expr_stop.
   Qed.
 
-  Lemma sim_tgt_rec_Load Π Φ l v `{!inMH _ Tgt nopMH Π} :
+  Lemma sim_tgt_rec_Load Π Φ l v :
     l ↦ v -∗
     (l ↦ v -∗ ▷ₒ Φ (Val v)) -∗
     TGT Load (Val (ValLoc l)) @ Π {{ Φ }}.
   Proof.
-    iIntros "Hl HΦ". iApply (sim_gen_expr_steps with "[-]") => /=.
+    iIntros "Hl HΦ". iApply (sim_gen_expr_steps_None with "[-]") => /=.
     iIntros ([e h0 fns0] ??) "[#Hfns [Hh Ha]]". simplify_eq/=.
     iDestruct (rec_mapsto_lookup with "[$] [$]") as %?.
     iApply (sim_tgt_step_end with "[-]"). iIntros (?? Hp). simplify_eq/=.
@@ -179,16 +178,16 @@ Section lifting.
     { done. }
     move => [? [Hstep ?]]. inv Hstep.
     iSpecialize ("HΦ" with "[$]").
-    iModIntro. iSplit!. do 2 iModIntro. iApply (inMH_apply nopMH with "[-]"). iSplit!. iFrame "∗#".
-    by iApply sim_gen_expr_end.
+    iModIntro. iSplit!. do 2 iModIntro. iSplit!. iFrame "∗#".
+    by iApply sim_gen_expr_stop.
   Qed.
 
-  Lemma sim_tgt_rec_Store Π Φ l v v' `{!inMH _ Tgt nopMH Π} :
+  Lemma sim_tgt_rec_Store Π Φ l v v' :
     l ↦ v -∗
     (l ↦ v' -∗ ▷ₒ Φ (Val v')) -∗
     TGT Store (Val (ValLoc l)) (Val v') @ Π {{ Φ }}.
   Proof.
-    iIntros "Hl HΦ". iApply (sim_gen_expr_steps with "[-]") => /=.
+    iIntros "Hl HΦ". iApply (sim_gen_expr_steps_None with "[-]") => /=.
     iIntros ([e h0 fns0] ??) "[#Hfns [Hh Ha]]". simplify_eq/=.
     iDestruct (rec_mapsto_lookup with "[$] [$]") as %?.
     iApply (sim_tgt_step_end with "[-]"). iIntros (?? Hp). simplify_eq/=.
@@ -198,18 +197,18 @@ Section lifting.
     move => [? [Hstep ?]]. inv Hstep.
     iMod (rec_mapsto_update with "[$] [$]") as "[??]".
     iSpecialize ("HΦ" with "[$]").
-    iModIntro. iSplit!. { by eexists. } do 2 iModIntro. iApply (inMH_apply nopMH with "[-]"). iSplit!.
-    iFrame "∗#" => /=. rewrite dom_alter_L. iFrame. by iApply sim_gen_expr_end.
+    iModIntro. iSplit!. { by eexists. } do 2 iModIntro. iSplit!.
+    iFrame "∗#" => /=. rewrite dom_alter_L. iFrame. by iApply sim_gen_expr_stop.
   Qed.
 
-  Lemma sim_tgt_rec_AllocA e Π Φ vs `{!inMH _ Tgt nopMH Π} :
+  Lemma sim_tgt_rec_AllocA e Π Φ vs :
     Forall (λ z, 0 < z) vs.*2 →
     (∀ ls, ([∗ list] l;n∈ls; vs.*2, [∗ list] o∈seqZ 0 n, (l +ₗ o) ↦ 0) -∗
      ▷ₒ TGT subst_l vs.*1 (ValLoc <$> ls) e @ Π {{ e',
      ∃ v, ⌜e' = Val v⌝ ∗ ([∗ list] l;n∈ls; vs.*2, [∗ list] o∈seqZ 0 n, ∃ v, (l +ₗ o) ↦ v) ∗ Φ e' }}) -∗
     TGT AllocA vs e @ Π {{ Φ }}.
   Proof.
-    iIntros (Hall) "HΦ". iApply (sim_gen_expr_steps with "[-]") => /=.
+    iIntros (Hall) "HΦ". iApply (sim_gen_expr_steps_None with "[-]") => /=.
     iIntros ([? h0 fns0] ??) "[#Hfns [Hh Ha]]". simplify_eq/=.
     iApply (sim_tgt_step_end with "[-]"). iIntros (?? Hp). simplify_eq/=.
     exploit prim_step_inv_head; [done|..].
@@ -219,13 +218,13 @@ Section lifting.
     iMod (rec_mapsto_alloc_list with "Hh") as "[Hh ?]"; [done|].
     iMod (rec_alloc_alloc_list with "Ha") as "[Ha Has]"; [done..|].
     iSpecialize ("HΦ" with "[$]").
-    iModIntro. iSplit!. do 2 iModIntro. iApply (inMH_apply nopMH with "[-]"). iSplit!.
+    iModIntro. iSplit!. do 2 iModIntro. iSplit!.
     iFrame "∗#" => /=.
 
     iApply (sim_gen_expr_bind _ [FreeACtx _] _ with "[-]") => /=.
     iApply (sim_gen_expr_wand with "HΦ") => /=.
     iIntros (?) "[% [% [Hl HΦ]]]" => /=. simplify_eq/=.
-    iApply (sim_gen_expr_steps with "[-]") => /=.
+    iApply (sim_gen_expr_steps_None with "[-]") => /=.
     iIntros ([? h1 fns1] ??) "[#Hfns1 [Hh Ha]]". simplify_eq/=.
     iApply (sim_tgt_step_end with "[-]"). iIntros (???). simplify_eq/=.
     exploit prim_step_inv_head; [done|..].
@@ -233,37 +232,37 @@ Section lifting.
     { done. }
     move => [? [Hstep ?]]. inv Hstep.
     iMod (rec_alloc_free_list with "Hh Ha [$] [$]") as (??) "[??]".
-    iModIntro. iSplit!. { done. } do 2 iModIntro. iApply (inMH_apply nopMH with "[-]"). iSplit!.
-    iFrame "∗#" => /=. by iApply sim_gen_expr_end.
+    iModIntro. iSplit!. { done. } do 2 iModIntro. iSplit!.
+    iFrame "∗#" => /=. by iApply sim_gen_expr_stop.
   Qed.
 
-  Lemma sim_tgt_rec_LetE Π Φ s v e `{!inMH _ Tgt nopMH Π} :
+  Lemma sim_tgt_rec_LetE Π Φ s v e :
     (▷ₒ TGT (subst s v e) @ Π {{ Φ }}) -∗
     TGT LetE s (Val v) e @ Π {{ Φ }}.
   Proof.
-    iIntros "HΦ". iApply (sim_gen_expr_steps with "[-]") => /=.
+    iIntros "HΦ". iApply (sim_gen_expr_steps_None with "[-]") => /=.
     iIntros ([? h0 fns0] ??) "[#Hfns [Hh Ha]]". simplify_eq/=.
     iApply (sim_tgt_step_end with "[-]"). iIntros (?? Hp). simplify_eq/=.
     exploit prim_step_inv_head; [done|..].
     { apply sub_redexes_are_values_item; case; naive_solver. }
     { done. }
     move => [? [Hstep ?]]. inv Hstep.
-    iModIntro. iSplit!. do 2 iModIntro. iApply (inMH_apply nopMH with "[-]"). iSplit!.
+    iModIntro. iSplit!. do 2 iModIntro. iSplit!.
     iFrame "∗#" => /=.
   Qed.
 
-  Lemma sim_tgt_rec_If Π Φ (b : bool) e1 e2 `{!inMH _ Tgt nopMH Π} :
+  Lemma sim_tgt_rec_If Π Φ (b : bool) e1 e2 :
     (▷ₒ TGT (if b then e1 else e2) @ Π {{ Φ }}) -∗
     TGT If (Val (ValBool b)) e1 e2 @ Π {{ Φ }}.
   Proof.
-    iIntros "HΦ". iApply (sim_gen_expr_steps with "[-]") => /=.
+    iIntros "HΦ". iApply (sim_gen_expr_steps_None with "[-]") => /=.
     iIntros ([? h0 fns0] ??) "[#Hfns [Hh Ha]]". simplify_eq/=.
     iApply (sim_tgt_step_end with "[-]"). iIntros (?? Hp). simplify_eq/=.
     exploit prim_step_inv_head; [done|..].
     { apply sub_redexes_are_values_item; case; naive_solver. }
     { done. }
     move => [? [Hstep ?]]. inv Hstep.
-    iModIntro. iSplit!. do 2 iModIntro. iApply (inMH_apply nopMH with "[-]"). iSplit!.
+    iModIntro. iSplit!. do 2 iModIntro. iSplit!.
     iFrame "∗#" => /=.
   Qed.
 
@@ -272,7 +271,7 @@ End lifting.
 Section memmove.
   Context `{!dimsumGS Σ} `{!recGS Σ}.
 
-  Lemma sim_memcpy Π `{!inMH _ Tgt nopMH Π}:
+  Lemma sim_memcpy Π :
     "memcpy" ↪ Some memcpy_rec -∗
     rec_fn_spec_hoare Tgt Π "memcpy" (λ es POST,
       ∃ d s n o d' s' hvss hvsd, ⌜es = [Val $ ValLoc d; Val $ ValLoc s; Val $ ValNum n; Val $ ValNum o]⌝ ∗
@@ -293,7 +292,7 @@ Section memmove.
     iApply (sim_gen_expr_bind _ [IfCtx _ _] _ with "[-]") => /=.
     iApply sim_tgt_rec_BinOp; [done|]. iModIntro => /=.
     iApply sim_tgt_rec_If. iModIntro => /=. case_bool_decide (0 < _).
-    2: { destruct hvss, hvsd => //. iApply sim_gen_expr_end. iSplit!. iApply "HΦ". iSplit!. }
+    2: { destruct hvss, hvsd => //. iApply sim_gen_expr_stop. iSplit!. iApply "HΦ". iSplit!. }
     iApply (sim_gen_expr_bind _ [LetECtx _ _] with "[-]") => /=.
     iApply (sim_gen_expr_bind _ [StoreRCtx _] with "[-]") => /=.
     destruct Ho; simplify_eq; case_bool_decide => //.
@@ -421,7 +420,7 @@ Section memmove.
       ∃ l1 l2, ⌜es = [Val (ValLoc l1); Val $ ValLoc l2]⌝ ∗
        POST (λ v, ∃ b, ⌜v = ValBool b⌝ ∗ ⌜l1.1 = l2.1 → b = bool_decide (l1.2 ≤ l2.2)⌝).
 
-  Lemma sim_memmove Π `{!inMH _ Tgt nopMH Π}:
+  Lemma sim_memmove Π :
     "memmove" ↪ Some memmove_rec -∗
     "memcpy" ↪ Some memcpy_rec -∗
     □ rec_fn_spec_hoare Tgt Π "locle" locle_fn_spec -∗
@@ -441,7 +440,7 @@ Section memmove.
     iApply "Hlocle". iExists _, _. iSplit!. iIntros (? [b [-> Hb]]) => /=.
     iApply sim_tgt_rec_If. iModIntro => /=. destruct b.
     - iApply (sim_memcpy with "[//]"). iFrame. iSplit!. { case_bool_decide; naive_solver. }
-      iIntros (?) "[-> ?]". iSplit!. iApply sim_gen_expr_end. iApply ("HΦ" with "[-]"). by iFrame.
+      iIntros (?) "[-> ?]". iSplit!. iApply sim_gen_expr_stop. iApply ("HΦ" with "[-]"). by iFrame.
     - iApply (sim_gen_expr_bind _ [CallCtx _ [] _] with "[-]") => /=.
       iApply (sim_gen_expr_bind _ [BinOpRCtx _ _] with "[-]") => /=.
       iApply sim_tgt_rec_BinOp; [done|]. iModIntro => /=.
@@ -460,16 +459,15 @@ Section memmove.
         move => /Hb Hx. symmetry in Hx. rewrite bool_decide_eq_false in Hx.
         simpl. lia.
       }
-      iIntros (?) "[-> ?]". iSplit!. iApply sim_gen_expr_end. iApply ("HΦ" with "[-]"). by iFrame.
+      iIntros (?) "[-> ?]". iSplit!. iApply sim_gen_expr_stop. iApply ("HΦ" with "[-]"). by iFrame.
   Qed.
 
-  Local Canonical Structure spec_mod_lang_unit.
   (* This spec is tricky to use since one needs to pick one Π upfront *)
-  Lemma sim_locle_spec Π Φ :
-    (∀ f vs h σ, handle_cont _ Tgt Π (Some (Incoming, ERCall f vs h)) σ (λ σ', ∃ l1 l2, ⌜σ' = σ⌝ ∗
+  Lemma sim_locle_spec `{!specGS} Π Φ :
+    (∀ f vs h σ, switch_id Tgt _ Π (Some (Incoming, ERCall f vs h)) σ (λ σ', ∃ l1 l2, ⌜σ' = σ⌝ ∗
       ⌜f = "locle"⌝ ∗ ⌜vs = [ValLoc l1; ValLoc l2]⌝ ∗ (∀ b,
         ⌜l1.1 = l2.1 → b = bool_decide (l1.2 ≤ l2.2)⌝ -∗ ∀ σ,
-          handle_cont _ Tgt Π (Some (Outgoing, ERReturn (ValBool b) h)) σ (λ σ', ⌜σ' = σ⌝ ∗
+          switch_id Tgt _ Π (Some (Outgoing, ERReturn (ValBool b) h)) σ (λ σ', ⌜σ' = σ⌝ ∗
             TGT locle_spec @ Π {{ Φ }})))) -∗
     TGT locle_spec @ Π {{ Φ }}.
   Proof.
@@ -477,46 +475,48 @@ Section memmove.
     rewrite /TReceive bind_bind bind_bind.
     iApply (sim_tgt_TExist with "[-]"). iIntros ([[??]?]) "!>".
     rewrite bind_bind. setoid_rewrite bind_ret_l.
-    iApply (sim_gen_TVis with "[-]"). iIntros ([]) "!>".
-    iApply (handle_cont_mono with "HC"). iIntros (?). iDestruct 1 as (l1 l2 -> -> ->) "HC" => /=. iSplit; [done|].
+    iApply (sim_gen_TVis with "[-]"). iIntros ([]) "? !>".
+    iApply (switch_id_mono with "HC"). iIntros (?). iDestruct 1 as (l1 l2 -> -> ->) "HC" => /=. iFrame.
     rewrite bind_bind. iApply (sim_tgt_TAssume with "[-]"); [done|]. iIntros "!>".
     rewrite bind_bind. iApply (sim_tgt_TAll with "[-]"). iIntros "!>".
     rewrite bind_bind. iApply (sim_tgt_TAll with "[-]"). iIntros "!>".
     rewrite bind_bind. iApply (sim_tgt_TAssume with "[-]"); [done|]. iIntros "!>".
     rewrite bind_bind. iApply (sim_tgt_TExist with "[-]"). iIntros (b) "!>".
     rewrite bind_bind. iApply (sim_tgt_TAssert with "[-]"). iIntros (?) "!>".
-    iApply (sim_gen_TVis with "[-]"). iIntros ([]) "!>".
-    iApply (handle_cont_mono with "[HC]"). { iApply ("HC" with "[//]"). }
-    simpl. iIntros (?). iDestruct 1 as (->) "HC". iSplit; [done|].
-    done.
+    iApply (sim_gen_TVis with "[-]"). iIntros ([]) "? !>".
+    iApply (switch_id_mono with "[HC]"). { iApply ("HC" with "[//]"). }
+    simpl. iIntros (?). iDestruct 1 as (->) "HC". iFrame.
   Qed.
 
-  (* This spec does not require one to pick Π upfront, but it has the
-  downside that it is written in extreme continuation passing style *)
-  Lemma sim_locle_spec2 Π Φ :
-      (∀ f vs h σ C,
-        (∀ l1 l2 σ' Π' Φ',
-        ⌜σ' = σ⌝ -∗ ⌜f = "locle"⌝ -∗ ⌜vs = [ValLoc l1; ValLoc l2]⌝ -∗
-         (∀ b C', ⌜l1.1 = l2.1 → b = bool_decide (l1.2 ≤ l2.2)⌝ -∗
-         handle_cont (spec_trans _ _) Tgt Π' (Some (Outgoing, ERReturn (ValBool b) h)) (locle_spec, tt) C') -∗
-        TGT σ'.1 @ Π' {{ Φ' }}) -∗
-      handle_cont (spec_trans _ _) Tgt Π (Some (Incoming, ERCall f vs h)) σ C) -∗
+  (* This spec does not require one to pick Π upfront *)
+  Lemma sim_locle_spec2 `{!specGS} Π Φ :
+    switch Π (λ κ σ POST,
+      ∃ f vs h, ⌜κ = Some (Incoming, ERCall f vs h)⌝ ∗
+    POST Tgt (spec_trans _ unit) (λ σ' Π',
+      ∃ l1 l2, ⌜σ' = σ⌝ ∗ ⌜f = "locle"⌝ ∗ ⌜vs = [ValLoc l1; ValLoc l2]⌝ ∗
+    switch Π' (λ κ σ POST,
+      ∃ b, ⌜l1.1 = l2.1 → b = bool_decide (l1.2 ≤ l2.2)⌝ ∗
+      ⌜κ = (Some (Outgoing, ERReturn (ValBool b) h))⌝ ∗ ⌜σ = (locle_spec, tt)⌝ ∗
+      spec_state ()
+      ))) -∗
     TGT locle_spec @ Π {{ Φ }}.
   Proof.
     iDestruct 1 as "HC". unfold locle_spec at 2. rewrite unfold_forever -/locle_spec.
     rewrite /TReceive bind_bind bind_bind.
     iApply (sim_tgt_TExist with "[-]"). iIntros ([[??]?]) "!>".
     rewrite bind_bind. setoid_rewrite bind_ret_l.
-    iApply (sim_gen_TVis with "[-]"). iIntros ([]) "!>".
-    iApply "HC". iIntros (????? -> -> ->) "HC". simpl.
+    iApply (sim_gen_TVis with "[-]"). iIntros ([]) "Hs !>".
+    iIntros (??) "[% [% _]]". subst.
+    iApply "HC". iSplit!. iIntros (??). iDestruct 1 as (?????) "HC". subst.
+    iApply (sim_gen_expr_intro _ tt with "[Hs]"); simpl; [done..|].
     rewrite bind_bind. iApply (sim_tgt_TAssume with "[-]"); [done|]. iIntros "!>".
     rewrite bind_bind. iApply (sim_tgt_TAll with "[-]"). iIntros "!>".
     rewrite bind_bind. iApply (sim_tgt_TAll with "[-]"). iIntros "!>".
     rewrite bind_bind. iApply (sim_tgt_TAssume with "[-]"); [done|]. iIntros "!>".
     rewrite bind_bind. iApply (sim_tgt_TExist with "[-]"). iIntros (b) "!>".
     rewrite bind_bind. iApply (sim_tgt_TAssert with "[-]"). iIntros (?) "!>".
-    iApply (sim_gen_TVis with "[-]"). iIntros ([]) "!>".
-    by iApply "HC".
+    iApply (sim_gen_TVis with "[-]"). iIntros ([]) "? !>".
+    iIntros (??) "[% [% _]]". subst. iApply "HC". iSplit!.
   Qed.
 
 (*
@@ -554,15 +554,15 @@ Section memmove.
   Qed.
 *)
 
-  Program Definition locleMH m1 : iModHandler Σ (m_state m1) rec_event := {|
-    imodhandle κ σ C := ∀ fns1 Π_s s,
-      let Π := (link_tgt_leftP (m2:=spec_trans _ _) (rec_link_filter fns1 {["locle"]}) Π_s s (locle_spec, tt)) in
-        (∀ σ', C σ' -∗ σ' ≈{ m1 }≈>ₜ Π) -∗ Π κ σ
-  |}%I.
-  Next Obligation.
-    simpl. iIntros (?????) "HP HC". iIntros (???) "Hw". iApply "HP". iIntros (?) "?".
-    iApply "Hw". by iApply "HC".
-  Qed.
+  (* Program Definition locleMH m1 : iModHandler Σ (m_state m1) rec_event := {| *)
+  (*   imodhandle κ σ C := ∀ fns1 Π_s s, *)
+  (*     let Π := (link_tgt_leftP (m2:=spec_trans _ _) (rec_link_filter fns1 {["locle"]}) Π_s s (locle_spec, tt)) in *)
+  (*       (∀ σ', C σ' -∗ σ' ≈{ m1 }≈>ₜ Π) -∗ Π κ σ *)
+  (* |}%I. *)
+  (* Next Obligation. *)
+  (*   simpl. iIntros (?????) "HP HC". iIntros (???) "Hw". iApply "HP". iIntros (?) "?". *)
+  (*   iApply "Hw". by iApply "HC". *)
+  (* Qed. *)
 
   (* Program Definition locleMH m1 : iModHandler Σ (m_state m1) rec_event := {| *)
   (*   imodhandle κ σ C := ∀ fns1 Π_s γ_s γσ_locle (s : list seq_product_case),  *)
@@ -577,91 +577,102 @@ Section memmove.
 
 
 
-  Lemma sim_locle fns Π `{!inMH _ Tgt (locleMH _) Π}:
-    rec_fn_auth fns -∗
-    "locle" ↪ None -∗
-    rec_fn_spec_hoare Tgt Π "locle" locle_fn_spec.
-  Proof.
-    iIntros "#Hfns #Hf" (es Φ) "HΦ". iDestruct "HΦ" as (l1 l2 ->) "HΦ".
-    iApply (sim_tgt_rec_Call_external with "[$]"). iIntros (???) "#??? !>".
-    iApply (inMH_apply (locleMH _)). iIntros (???) "Hσ".
-    iIntros (??????). destruct!/=. case_bool_decide => //. rewrite (bool_decide_true (_ ∈ _)) //.
-    iApply (sim_tgt_link_right_recv with "[-]").
-    iApply (sim_gen_expr_intro _ tt _ None); simpl; [done..|].
-    (* iApply sim_locle_spec => /=. iIntros (????) "Hc". iIntros (?). simplify_eq/=. *)
-    unfold locle_spec at 2. rewrite unfold_forever -/locle_spec.
-    rewrite /TReceive bind_bind bind_bind.
-    iApply (sim_tgt_TExist with "[-]"). iIntros ([[??]?]) "!>".
-    rewrite bind_bind. setoid_rewrite bind_ret_l.
-    iApply (sim_gen_TVis with "[-]").
-    iIntros (?) "!>". simpl. iIntros "_" (?). simplify_eq/=.
-    iApply (sim_tgt_link_right with "[-]").
-    iApply (sim_gen_expr_intro _ tt _ None); simpl; [done..|].
-    rewrite bind_bind. iApply (sim_tgt_TAssume with "[-]"); [done|]. iIntros "!>".
-    rewrite bind_bind. iApply (sim_tgt_TAll with "[-]"). iIntros "!>".
-    rewrite bind_bind. iApply (sim_tgt_TAll with "[-]"). iIntros "!>".
-    rewrite bind_bind. iApply (sim_tgt_TAssume with "[-]"); [done|]. iIntros "!>".
-    rewrite bind_bind. iApply (sim_tgt_TExist with "[-]"). iIntros (b) "!>".
-    rewrite bind_bind. iApply (sim_tgt_TAssert with "[-]"). iIntros (?) "!>".
-    iApply (sim_gen_TVis with "[-]"). iIntros (?) "!> _".
-    iIntros (??????). destruct!/=.
-    iApply (sim_tgt_link_left_recv with "[-]").
-    iApply sim_tgt_rec_Waiting_raw.
-    iSplit. { iIntros. iModIntro. iIntros (?). simplify_eq. }
-    iIntros (???) "!>". iIntros (?). iApply (sim_tgt_link_left with "[-]"). destruct_all unit.
-    iApply "Hσ". simplify_eq/=. iExists _. iFrame. iSplit!. iApply "HΦ". iSplit!.
-  Qed.
+  (* Lemma sim_locle fns Π `{!inMH _ Tgt (locleMH _) Π}: *)
+  (*   rec_fn_auth fns -∗ *)
+  (*   "locle" ↪ None -∗ *)
+  (*   rec_fn_spec_hoare Tgt Π "locle" locle_fn_spec. *)
+  (* Proof. *)
+  (*   iIntros "#Hfns #Hf" (es Φ) "HΦ". iDestruct "HΦ" as (l1 l2 ->) "HΦ". *)
+  (*   iApply (sim_tgt_rec_Call_external with "[$]"). iIntros (???) "#??? !>". *)
+  (*   iApply (inMH_apply (locleMH _)). iIntros (???) "Hσ". *)
+  (*   iIntros (??????). destruct!/=. case_bool_decide => //. rewrite (bool_decide_true (_ ∈ _)) //. *)
+  (*   iApply (sim_tgt_link_right_recv with "[-]"). *)
+  (*   iApply (sim_gen_expr_intro _ tt _ None); simpl; [done..|]. *)
+  (*   (* iApply sim_locle_spec => /=. iIntros (????) "Hc". iIntros (?). simplify_eq/=. *) *)
+  (*   unfold locle_spec at 2. rewrite unfold_forever -/locle_spec. *)
+  (*   rewrite /TReceive bind_bind bind_bind. *)
+  (*   iApply (sim_tgt_TExist with "[-]"). iIntros ([[??]?]) "!>". *)
+  (*   rewrite bind_bind. setoid_rewrite bind_ret_l. *)
+  (*   iApply (sim_gen_TVis with "[-]"). *)
+  (*   iIntros (?) "!>". simpl. iIntros "_" (?). simplify_eq/=. *)
+  (*   iApply (sim_tgt_link_right with "[-]"). *)
+  (*   iApply (sim_gen_expr_intro _ tt _ None); simpl; [done..|]. *)
+  (*   rewrite bind_bind. iApply (sim_tgt_TAssume with "[-]"); [done|]. iIntros "!>". *)
+  (*   rewrite bind_bind. iApply (sim_tgt_TAll with "[-]"). iIntros "!>". *)
+  (*   rewrite bind_bind. iApply (sim_tgt_TAll with "[-]"). iIntros "!>". *)
+  (*   rewrite bind_bind. iApply (sim_tgt_TAssume with "[-]"); [done|]. iIntros "!>". *)
+  (*   rewrite bind_bind. iApply (sim_tgt_TExist with "[-]"). iIntros (b) "!>". *)
+  (*   rewrite bind_bind. iApply (sim_tgt_TAssert with "[-]"). iIntros (?) "!>". *)
+  (*   iApply (sim_gen_TVis with "[-]"). iIntros (?) "!> _". *)
+  (*   iIntros (??????). destruct!/=. *)
+  (*   iApply (sim_tgt_link_left_recv with "[-]"). *)
+  (*   iApply sim_tgt_rec_Waiting_raw. *)
+  (*   iSplit. { iIntros. iModIntro. iIntros (?). simplify_eq. } *)
+  (*   iIntros (???) "!>". iIntros (?). iApply (sim_tgt_link_left with "[-]"). destruct_all unit. *)
+  (*   iApply "Hσ". simplify_eq/=. iExists _. iFrame. iSplit!. iApply "HΦ". iSplit!. *)
+  (* Qed. *)
 
 
-  Definition locleMH1 m1 Π Πi : iModHandler Σ (m_state m1) rec_event :=
-    switchMH Π (λ κ σ C, ∃ vs h, ⌜κ = Some (Outgoing, ERCall "locle" vs h)⌝ ∗
-      C Tgt (spec_trans _ unit) (locle_spec, tt) Πi)%I.
+  (* Definition locleMH1 m1 Π Πi : iModHandler Σ (m_state m1) rec_event := *)
+  (*   switchMH Π (λ κ σ C, ∃ vs h, ⌜κ = Some (Outgoing, ERCall "locle" vs h)⌝ ∗ *)
+  (*     C Tgt (spec_trans _ unit) (locle_spec, tt) Πi)%I. *)
 
-  Definition locleMH2 {S} Πi Πr : iModHandler Σ (m_state (spec_trans _ S)) rec_event :=
-    switchMH Πi (λ κ σ C, ∃ f vs h, ⌜κ = Some (Incoming, ERCall f vs h)⌝ ∗
-      C Tgt (spec_trans _ S) σ Πr)%I.
+  (* Definition locleMH2 {S} Πi Πr : iModHandler Σ (m_state (spec_trans _ S)) rec_event := *)
+  (*   switchMH Πi (λ κ σ C, ∃ f vs h, ⌜κ = Some (Incoming, ERCall f vs h)⌝ ∗ *)
+  (*     C Tgt (spec_trans _ S) σ Πr)%I. *)
 
-  Definition switch_spec {S EV} (Π : option EV → S → iProp Σ)
-    (K : option EV → S → (tgt_src → ∀ m : mod_trans EV, _ →_ → iProp Σ) → iProp Σ) : iProp Σ :=
-    (∀ κ σ, K κ σ (λ ts' m' σ' PΠ', ∀ Π', PΠ' Π' -∗ σ' ≈{ ts', m' }≈> Π') -∗  Π κ σ).
+  (* internal *)
+  Definition switch_link_int {S EV} (ts : tgt_src) (m2 : mod_trans (io_event EV)) (Π : option (io_event EV) → S → iProp Σ)
+    (K : _) : iProp Σ :=
+    switch Π (λ κ σ0 POST,
+      K σ0 (λ e σ2 K2, ⌜κ = Some (Outgoing, e)⌝ ∗
+    POST ts m2 (λ σi Πi,
+      ⌜σi = σ2⌝ ∗
+    switch Πi (λ κ' σ POST,
+      ∃ e', ⌜κ' = Some (Incoming, e')⌝ ∗
+    POST ts m2 (λ σr Πr,
+      ⌜σr = σ⌝ ∗ ⌜e' = e⌝ ∗ K2 σ Πr)))))%I.
+
 
   Lemma sim_locle2 fns Π :
     rec_fn_auth fns -∗
     "locle" ↪ None -∗
-    switch_spec Π (λ κ σ0 C, ∃ vs h, ⌜κ = Some (Outgoing, ERCall "locle" vs h)⌝ ∗
-      C Tgt (spec_trans _ _) (locle_spec, tt) (λ Πi,
-       switch_spec Πi (λ κ' σ C, ∃ e, ⌜κ' = Some (Incoming, e)⌝ ∗
-         (⌜e = ERCall "locle" vs h⌝ -∗ C Tgt _ σ (λ Πr,
-          switch_spec Πr (λ κ'' σ C, ∃ v h', ⌜κ'' = Some (Outgoing, ERReturn v h')⌝ ∗ ⌜σ = (locle_spec, tt)⌝ ∗
-              C Tgt _ σ0 (λ Πf,
-               (switch_spec Πf (λ κ σ C, ∃ e, ⌜κ = Some (Incoming, e)⌝ ∗
-                     (⌜e = ERReturn v h'⌝ -∗ C Tgt _ σ (λ Πx, ⌜Πx = Π⌝))))
-      ))))))) -∗
+    switch Π (λ κ σ0 POST,
+      ∃ vs h, ⌜κ = Some (Outgoing, ERCall "locle" vs h)⌝ ∗
+    POST Tgt (spec_trans _ _) (λ σi Πi,
+      ⌜σi = (locle_spec, tt)⌝ ∗
+    switch Πi (λ κ' σ POST,
+      ∃ e, ⌜κ' = Some (Incoming, e)⌝ ∗
+    POST Tgt _ (λ σr Πr,
+      ⌜σr = σ⌝ ∗ ⌜e = ERCall "locle" vs h⌝ ∗
+    switch Πr (λ κ'' σ POST,
+      ∃ v h', ⌜κ'' = Some (Outgoing, ERReturn v h')⌝ ∗ ⌜σ = (locle_spec, tt)⌝ ∗
+    POST Tgt _ (λ σf Πf,
+      ⌜σf = σ0⌝ ∗
+    switch Πf (λ κ σ POST,
+      ∃ e, ⌜κ = Some (Incoming, e)⌝ ∗
+    POST Tgt rec_trans (λ σx Πx,
+      ⌜e = ERReturn v h'⌝ ∗ ⌜σx = σ⌝ ∗ ⌜Πx = Π⌝)))))))) -∗
     rec_fn_spec_hoare Tgt Π "locle" locle_fn_spec.
   Proof.
     iIntros "#Hfns #Hf HΠ" (es Φ) "HΦ". iDestruct "HΦ" as (l1 l2 ->) "HΦ".
     iApply (sim_tgt_rec_Call_external with "[$]"). iIntros (???) "#??? !>".
-    iIntros "Hσ". iApply "HΠ". iSplit!. iIntros (?) "HΠi".
-    iApply (sim_gen_expr_intro _ tt _ None); simpl; [done..|].
+    iIntros (??) "[% [% Hσ]]". subst. iApply "HΠ". iSplit!. iIntros (??) "[-> HΠi]".
+    iApply (fupd_sim_gen with "[-]").
+    iMod (mstate_var_alloc unit) as (γ) "?".
+    iMod (mstate_var_split γ tt with "[$]") as "[Hγ ?]".
+    iModIntro.
+    pose (Hspec := SpecGS γ).
+    iApply (sim_gen_expr_intro _ tt with "[Hγ]"); simpl; [done..|].
     (* iApply sim_locle_spec2 => /=. iIntros (?????) "Hc _". iIntros (?). simplify_eq/=. *)
-    iApply sim_locle_spec2 => /=. iIntros (?????) "Hc".
-    iIntros "_". iApply "HΠi". iSplit!. iIntros (??) "HΠr". simplify_eq/=.
-    iApply (sim_gen_expr_intro _ tt _ None); simpl; [done..|].
-    iApply "Hc"; [done..|].
-    iIntros (???). iIntros "_". iApply "HΠr". iSplit!. iIntros (?) "HΠf".
+    iApply sim_locle_spec2 => /=. iIntros (??). iDestruct 1 as (????) "HC". subst.
+    iApply "HΠi". iSplit!. iIntros (??) "[% [% HΠr]]". simplify_eq/=.
+    iApply "HC". iSplit!. iIntros (??). iDestruct 1 as (????) "HC".
+    iApply "HΠr". iSplit!. iIntros (??) "[% HΠf]". simplify_eq.
     iApply sim_tgt_rec_Waiting_raw.
-    iSplit. { iIntros. iModIntro. iApply "HΠf". iSplit!. iIntros (?). simplify_eq. }
-    iIntros (???) "!>". iApply "HΠf". iSplit!. iIntros (???). simplify_eq.
-    iApply "Hσ". simplify_eq/=. iSplit!. iFrame. iApply "HΦ". iSplit!.
-    (* iApply "Hσ". iSplit!. iFrame. *)
-    (* iApply "HC". iIntros (?) "HC". *)
-    (* iIntros (??????). destruct!/=. *)
-    (* (* iApply (sim_tgt_link_left_recv with "[-]"). *) *)
-    (* iApply sim_tgt_rec_Waiting_raw. *)
-    (* iSplit. { iIntros. iModIntro. iApply "HC". iIntros (? ?). simplify_eq. } *)
-    (* iIntros (???) "!>". iApply "HC". iIntros (?). *)
-    (* iApply "Hσ". simplify_eq/=. *)
-(* iExists _. iFrame. iSplit!. by iApply "HΦ". *)
+    iSplit. { iIntros. iModIntro. iApply "HΠf". iSplit!. iIntros (??) "[% ?]". simplify_eq. }
+    iIntros (???) "!>". iApply "HΠf". iSplit!. iIntros (??[?[??]]). simplify_eq.
+    iApply "Hσ". iSplit!. iFrame. iApply "HΦ". iSplit!.
   Qed.
 
 (*
@@ -687,7 +698,7 @@ Hoare triple spec:
 *)
 
 
-  Lemma sim_main Π `{!inMH _ Tgt nopMH Π}:
+  Lemma sim_main Π :
     "memmove" ↪ Some memmove_rec -∗
     "memcpy" ↪ Some memcpy_rec -∗
     "main" ↪ Some main_rec -∗
@@ -756,7 +767,7 @@ Hoare triple spec:
     iApply "HΦ". iSplit!. iIntros (?) "HΦ".
 
     iApply (sim_tgt_rec_LetE with "[-]"). iIntros "!>" => /=.
-    iApply sim_gen_expr_end => /=. iSplit!. iFrame. by iApply "HΦ".
+    iApply sim_gen_expr_stop => /=. iSplit!. iFrame. by iApply "HΦ".
   Qed.
 
   Definition main_spec_body : spec rec_event unit void :=
@@ -773,7 +784,7 @@ Hoare triple spec:
     TUb.
 
 
-  Lemma sim_main_full Π γσ_s (σ : m_state (spec_trans _ unit)) `{!inMH _ Tgt nopMH Π}:
+  Lemma sim_main_full Π γσ_s (σ : m_state (spec_trans _ unit)) :
     "memmove" ↪ Some memmove_rec -∗
     "memcpy" ↪ Some memcpy_rec -∗
     "main" ↪ Some main_rec -∗
@@ -783,137 +794,148 @@ Hoare triple spec:
     ⌜σ.1 ≡ main_spec_body⌝ -∗
     rec_fn_spec_hoare Tgt Π "main" (λ es POST,
       ⌜es = []⌝ ∗
-      □ switch_spec Π (λ κ σ POST,
+      □ switch Π (λ κ σ POST,
           ∃ vs h σ_s, ⌜κ = Some (Outgoing, ERCall "print" vs h)⌝ ∗ γσ_s ⤳ σ_s ∗
-          POST Src (spec_trans _ unit) σ_s (λ Π_s,
-
-          switch_spec Π_s (λ κ' σ_s2 POST,
+        POST Src (spec_trans _ unit) (λ σ_s' Π_s,
+          ⌜σ_s' = σ_s⌝ ∗
+        switch Π_s (λ κ' σ_s2 POST,
           ⌜κ' = κ⌝ ∗
-          POST Src _ σ_s2 (λ Π',
-
-          ∃ e,
-          switch_spec Π' (λ κ'' σ_s3 POST,
+        POST Src _ (λ σ_s2' Π',
+          ∃ e, ⌜σ_s2' = σ_s2⌝ ∗
+        switch Π' (λ κ'' σ_s3 POST,
           ⌜κ'' = Some (Incoming, e)⌝ ∗
-          POST Src _ σ_s3 (λ Π_s'',
-
-          switch_spec Π_s'' (λ κ'' σ'' POST,
+        POST Src _ (λ σ_s3' Π_s'',
+          ⌜σ_s3' = σ_s3⌝ ∗
+        switch Π_s'' (λ κ'' σ'' POST,
           ∃ v h', ⌜e = ERReturn v h'⌝ ∗ ⌜κ'' = None⌝ ∗
-          POST Tgt _ σ (λ Π',
-
-          γσ_s ⤳ σ'' ∗
-          switch_spec Π' (λ κ σ POST,
+        POST Tgt _ (λ σ' Π',
+          ⌜σ' = σ⌝ ∗ γσ_s ⤳ σ'' ∗
+        switch Π' (λ κ σ POST,
           ∃ e', ⌜κ = Some (Incoming, e')⌝ ∗
-          POST Tgt _ σ (λ Π',
-
-          ⌜e = e'⌝ ∗ ⌜Π = Π'⌝)))))))))) ∗
+        POST Tgt _ (λ σ' Π',
+          ⌜σ' = σ⌝ ∗ ⌜e = e'⌝ ∗ ⌜Π = Π'⌝)))))))))) ∗
       POST (λ vr, ∃ σ_s, γσ_s ⤳ σ_s ∗ (∀ Π, σ_s ≈{ spec_trans rec_event () }≈>ₛ Π) ∗ ⌜vr = 0⌝)).
   Proof.
-    set (X := (switch_spec _) _).
+    set (X := (switch _) _).
     iIntros "#?#?#?#?#? Hσs". iIntros (??). iDestruct 1 as (?) "[#Hs Hend]".
+    iApply (fupd_sim_gen_expr with "[-]").
+    iMod (mstate_var_alloc unit) as (γ) "?".
+    iMod (mstate_var_split γ σ.2 with "[$]") as "[Hγ ?]".
+    iModIntro.
+    pose (Hspec := SpecGS γ).
+
     iApply sim_main; [done..|]. iSplit!.
 
     iIntros (??). iDestruct 1 as (->) "HΦ".
     iApply (sim_tgt_rec_Call_external); [done|].
-    iIntros (???) "Hfns' Hh Ha !>". iIntros "Hσ".
-    iApply "Hs". iSplit!. iFrame. iIntros (?) "HC".
-    iApply (sim_gen_expr_intro _ tt _ None with "[] [-]"); [simpl; done..|].
+    iIntros (???) "Hfns' Hh Ha !>". iIntros (??) "[-> [-> Hσ]]".
+    iApply "Hs". iSplit!. iFrame. iIntros (??) "[-> HC]".
+    iApply (sim_gen_expr_intro _ tt with "[Hγ] [-]"); simpl; [done..|].
     unfold main_spec_body.
     iApply (sim_src_TExist _).
-    iApply sim_gen_TVis. iIntros ([]) "_".
-    iApply "HC". iSplit!. iIntros (?) "[% HC]".
-    iApply (sim_gen_expr_intro _ tt _ None with "[] [-]"); [simpl; done..|].
+    iApply sim_gen_TVis. iIntros ([]) "Hγ".
+    iIntros (??) "[-> [-> ?]]".
+    iApply "HC". iSplit!. iIntros (??) "[% [-> HC]]".
+    iApply (sim_gen_expr_intro _ tt with "[Hγ] [-]"); [simpl; done..|].
     iApply (sim_src_TExist _).
-    iApply sim_gen_TVis. iIntros ([]) "_".
-    iApply "HC". iSplit!. iIntros (?) "HC".
-    iApply (sim_gen_expr_intro _ tt _ None with "[] [-]"); [simpl; done..|].
+    iApply sim_gen_TVis. iIntros ([]) "Hγ".
+    iIntros (??) "[-> [-> ?]]".
+    iApply "HC". iSplit!. iIntros (??) "[-> HC]".
+    iApply (sim_gen_expr_intro _ tt with "[Hγ] [-]"); [simpl; done..|].
     iApply sim_src_TAssume. iIntros (?). case_match => //; simplify_eq/=.
-    iApply sim_gen_expr_None => /=. iIntros (? [] ??) "_".
-    iApply "HC". iSplit!. iIntros (?) "[? HC]".
+    iApply sim_gen_expr_steps => /=. iIntros (? [] ?) "Hγ".
+    iApply (sim_gen_stop with "[-]").
+    iIntros (??) "[-> [-> ?]]".
+    iApply "HC". iSplit!. iIntros (??) "[-> [? HC]]".
     iApply sim_tgt_rec_Waiting_raw.
-    iSplit. { iIntros. iModIntro. iApply "HC". iSplit!. iIntros (?) "[% %]". simplify_eq. }
-    iIntros (?? _) "!>". iApply "HC". iSplit!. iIntros (?[??]). simplify_eq/=.
+    iSplit. { iIntros. iModIntro. iApply "HC". iSplit!. iIntros (??) "[% [% %]]". simplify_eq. }
+    iIntros (?? _) "!>". iApply "HC". iSplit!. iIntros (??[?[??]]). simplify_eq/=.
     iApply "Hσ". iSplit!. iFrame. iApply "HΦ".
 
     iIntros (??). iDestruct 1 as (->) "HΦ".
     iApply (sim_tgt_rec_Call_external); [done|].
-    iIntros (???) "Hfns'' Hh Ha !>". iIntros "Hσ".
-    iApply "Hs". iSplit!. iFrame. iIntros (?) "HC".
-    iApply (sim_gen_expr_intro _ tt _ None with "[] [-]"); [simpl; done..|].
+    iIntros (???) "Hfns'' Hh Ha !>". iIntros (??) "[-> [-> Hσ]]".
+    iApply "Hs". iSplit!. iFrame. iIntros (??) "[-> HC]".
+    iApply (sim_gen_expr_intro _ tt with "[Hγ] [-]"); simpl; [done..|].
+    unfold main_spec_body.
     iApply (sim_src_TExist _).
-    iApply sim_gen_TVis. iIntros ([]) "_".
-    iApply "HC". iSplit!. iIntros (?) "[% HC]".
-    iApply (sim_gen_expr_intro _ tt _ None with "[] [-]"); [simpl; done..|].
+    iApply sim_gen_TVis. iIntros ([]) "Hγ".
+    iIntros (??) "[-> [-> ?]]".
+    iApply "HC". iSplit!. iIntros (??) "[% [-> HC]]".
+    iApply (sim_gen_expr_intro _ tt with "[Hγ] [-]"); [simpl; done..|].
     iApply (sim_src_TExist _).
-    iApply sim_gen_TVis. iIntros ([]) "_".
-    iApply "HC". iSplit!. iIntros (?) "HC".
-    iApply (sim_gen_expr_intro _ tt _ None with "[] [-]"); [simpl; done..|].
+    iApply sim_gen_TVis. iIntros ([]) "Hγ".
+    iIntros (??) "[-> [-> ?]]".
+    iApply "HC". iSplit!. iIntros (??) "[-> HC]".
+    iApply (sim_gen_expr_intro _ tt with "[Hγ] [-]"); [simpl; done..|].
     iApply sim_src_TAssume. iIntros (?). case_match => //; simplify_eq/=.
-    iApply sim_gen_expr_None => /=. iIntros (? [] ??) "_".
-    iApply "HC". iSplit!. iIntros (?) "[? HC]".
+    iApply sim_gen_expr_steps => /=. iIntros (? [] ?) "Hγ".
+    iApply (sim_gen_stop with "[-]").
+    iIntros (??) "[-> [-> ?]]".
+    iApply "HC". iSplit!. iIntros (??) "[-> [? HC]]".
     iApply sim_tgt_rec_Waiting_raw.
-    iSplit. { iIntros. iModIntro. iApply "HC". iSplit!. iIntros (?[??]). simplify_eq. }
-    iIntros (?? _) "!>". iApply "HC". iSplit!. iIntros (?[??]). simplify_eq/=.
-    iApply "Hσ". iSplit!. iFrame. iApply "HΦ". iIntros (?) "->".
+    iSplit. { iIntros. iModIntro. iApply "HC". iSplit!. iIntros (??) "[% [% %]]". simplify_eq. }
+    iIntros (?? _) "!>". iApply "HC". iSplit!. iIntros (??[?[??]]). simplify_eq/=.
+    iApply "Hσ". iSplit!. iFrame. iApply "HΦ". iIntros (? ->).
 
     iApply ("Hend" with "[-]"). iFrame. iSplit!. iIntros (?).
-    iApply (sim_gen_expr_intro _ tt _ None with "[] [-]"); [simpl; done..|].
+    iApply (sim_gen_expr_intro _ tt with "[Hγ] [-]"); [simpl; done..|].
     iApply sim_src_TUb_end.
   Qed.
 
 
 
-  (* Writing this spec for main_spec probably does not gain much / if
-  anything compared to reasoning about the spec module directly *)
-  Lemma sim_main_spec Π Φ :
-    (∃ f vs h, ∀ σ, handle_cont _ Src Π (Some (Incoming, ERCall f vs h)) σ (λ σ', ⌜σ' = σ⌝ ∗ (
-      ⌜f = "main"⌝ -∗ ⌜vs = []⌝ -∗
-      ∀ σ, handle_cont _ Src Π None σ (λ σ', ⌜σ = σ'⌝ ∗
-      (∃ h', ∀ σ, handle_cont _ Src Π (Some (Outgoing, ERCall "print" [ValNum 1] h')) σ (λ σ', ⌜σ' = σ⌝ ∗
-      (∃ e, ∀ σ, handle_cont _ Src Π (Some (Incoming, e)) σ (λ σ', ⌜σ' = σ⌝ ∗ (∀ v', ⌜e = ERReturn v' h'⌝ -∗
-      ∀ σ, handle_cont _ Src Π None σ (λ σ', ⌜σ = σ'⌝ ∗
-      (∃ h', ∀ σ, handle_cont _ Src Π (Some (Outgoing, ERCall "print" [ValNum 2] h')) σ (λ σ', ⌜σ' = σ⌝ ∗
-      (∃ e, ∀ σ, handle_cont _ Src Π (Some (Incoming, e)) σ (λ σ', ⌜σ' = σ⌝ ∗ (∀ v', ⌜e = ERReturn v' h'⌝ -∗
-      ∀ σ, handle_cont _ Src Π None σ (λ σ', ⌜σ = σ'⌝ ∗ True)))))))))))))))) -∗
-    SRC main_spec @ Π {{ Φ }}.
-  Proof.
-    iIntros "HΦ". iDestruct "HΦ" as (f vs h) "HΦ".
-    iEval (unfold main_spec). rewrite /TReceive bind_bind.
-    iApply (sim_src_TExist (_, _, _)).
-    rewrite bind_bind. setoid_rewrite bind_ret_l.
-    iApply sim_gen_TVis. iIntros ([]). iApply (handle_cont_mono with "HΦ").
-    iIntros (?) "[-> HΦ]". iSplit; [done|].
-    iApply sim_src_TAssume. iIntros (?).
-    iApply sim_src_TAssume. iIntros (?). simplify_eq.
-    iDestruct ("HΦ" with "[//] [//]") as "HΦ".
-    iApply sim_gen_expr_None => /=. iIntros (? [] ??). iApply (handle_cont_mono with "HΦ").
-    iIntros (?) "[-> [% HΦ]]". iExists _. iSplit; [done|]. iSplit!.
-    iApply sim_src_TExist. iApply sim_gen_TVis. iIntros ([]). iApply (handle_cont_mono with "HΦ").
-    iIntros (?) "[-> [% HΦ]]". iSplit; [done|].
-    iApply sim_src_TExist. iApply sim_gen_TVis. iIntros ([]). iApply (handle_cont_mono with "HΦ").
-    iIntros (?) "[-> HΦ]". iSplit; [done|].
-    iApply sim_src_TAssume. iIntros (?). case_match => //; simplify_eq.
-    iDestruct ("HΦ" with "[//]") as "HΦ".
-    iApply sim_gen_expr_None => /=. iIntros (? [] ??). iApply (handle_cont_mono with "HΦ").
-    iIntros (?) "[-> [% HΦ]]". iExists _. iSplit; [done|]. iSplit!.
-    iApply sim_src_TExist. iApply sim_gen_TVis. iIntros ([]). iApply (handle_cont_mono with "HΦ").
-    iIntros (?) "[-> [% HΦ]]". iSplit; [done|].
-    iApply sim_src_TExist. iApply sim_gen_TVis. iIntros ([]). iApply (handle_cont_mono with "HΦ").
-    iIntros (?) "[-> HΦ]". iSplit; [done|].
-    iApply sim_src_TAssume. iIntros (?). case_match => //; simplify_eq.
-    iDestruct ("HΦ" with "[//]") as "HΦ".
-    iApply sim_gen_expr_None => /=. iIntros (? [] ??). iApply (handle_cont_mono with "HΦ").
-    iIntros (?) "[-> HΦ]". iExists _. iSplit; [done|]. iSplit!.
-    iApply sim_src_TUb_end.
-  Qed.
+  (* (* Writing this spec for main_spec probably does not gain much / if *)
+  (* anything compared to reasoning about the spec module directly *) *)
+  (* Lemma sim_main_spec Π Φ : *)
+  (*   (∃ f vs h, ∀ σ, handle_cont _ Src Π (Some (Incoming, ERCall f vs h)) σ (λ σ', ⌜σ' = σ⌝ ∗ ( *)
+  (*     ⌜f = "main"⌝ -∗ ⌜vs = []⌝ -∗ *)
+  (*     ∀ σ, handle_cont _ Src Π None σ (λ σ', ⌜σ = σ'⌝ ∗ *)
+  (*     (∃ h', ∀ σ, handle_cont _ Src Π (Some (Outgoing, ERCall "print" [ValNum 1] h')) σ (λ σ', ⌜σ' = σ⌝ ∗ *)
+  (*     (∃ e, ∀ σ, handle_cont _ Src Π (Some (Incoming, e)) σ (λ σ', ⌜σ' = σ⌝ ∗ (∀ v', ⌜e = ERReturn v' h'⌝ -∗ *)
+  (*     ∀ σ, handle_cont _ Src Π None σ (λ σ', ⌜σ = σ'⌝ ∗ *)
+  (*     (∃ h', ∀ σ, handle_cont _ Src Π (Some (Outgoing, ERCall "print" [ValNum 2] h')) σ (λ σ', ⌜σ' = σ⌝ ∗ *)
+  (*     (∃ e, ∀ σ, handle_cont _ Src Π (Some (Incoming, e)) σ (λ σ', ⌜σ' = σ⌝ ∗ (∀ v', ⌜e = ERReturn v' h'⌝ -∗ *)
+  (*     ∀ σ, handle_cont _ Src Π None σ (λ σ', ⌜σ = σ'⌝ ∗ True)))))))))))))))) -∗ *)
+  (*   SRC main_spec @ Π {{ Φ }}. *)
+  (* Proof. *)
+  (*   iIntros "HΦ". iDestruct "HΦ" as (f vs h) "HΦ". *)
+  (*   iEval (unfold main_spec). rewrite /TReceive bind_bind. *)
+  (*   iApply (sim_src_TExist (_, _, _)). *)
+  (*   rewrite bind_bind. setoid_rewrite bind_ret_l. *)
+  (*   iApply sim_gen_TVis. iIntros ([]). iApply (handle_cont_mono with "HΦ"). *)
+  (*   iIntros (?) "[-> HΦ]". iSplit; [done|]. *)
+  (*   iApply sim_src_TAssume. iIntros (?). *)
+  (*   iApply sim_src_TAssume. iIntros (?). simplify_eq. *)
+  (*   iDestruct ("HΦ" with "[//] [//]") as "HΦ". *)
+  (*   iApply sim_gen_expr_None => /=. iIntros (? [] ??). iApply (handle_cont_mono with "HΦ"). *)
+  (*   iIntros (?) "[-> [% HΦ]]". iExists _. iSplit; [done|]. iSplit!. *)
+  (*   iApply sim_src_TExist. iApply sim_gen_TVis. iIntros ([]). iApply (handle_cont_mono with "HΦ"). *)
+  (*   iIntros (?) "[-> [% HΦ]]". iSplit; [done|]. *)
+  (*   iApply sim_src_TExist. iApply sim_gen_TVis. iIntros ([]). iApply (handle_cont_mono with "HΦ"). *)
+  (*   iIntros (?) "[-> HΦ]". iSplit; [done|]. *)
+  (*   iApply sim_src_TAssume. iIntros (?). case_match => //; simplify_eq. *)
+  (*   iDestruct ("HΦ" with "[//]") as "HΦ". *)
+  (*   iApply sim_gen_expr_None => /=. iIntros (? [] ??). iApply (handle_cont_mono with "HΦ"). *)
+  (*   iIntros (?) "[-> [% HΦ]]". iExists _. iSplit; [done|]. iSplit!. *)
+  (*   iApply sim_src_TExist. iApply sim_gen_TVis. iIntros ([]). iApply (handle_cont_mono with "HΦ"). *)
+  (*   iIntros (?) "[-> [% HΦ]]". iSplit; [done|]. *)
+  (*   iApply sim_src_TExist. iApply sim_gen_TVis. iIntros ([]). iApply (handle_cont_mono with "HΦ"). *)
+  (*   iIntros (?) "[-> HΦ]". iSplit; [done|]. *)
+  (*   iApply sim_src_TAssume. iIntros (?). case_match => //; simplify_eq. *)
+  (*   iDestruct ("HΦ" with "[//]") as "HΦ". *)
+  (*   iApply sim_gen_expr_None => /=. iIntros (? [] ??). iApply (handle_cont_mono with "HΦ"). *)
+  (*   iIntros (?) "[-> HΦ]". iExists _. iSplit; [done|]. iSplit!. *)
+  (*   iApply sim_src_TUb_end. *)
+  (* Qed. *)
 End memmove.
 
 Section memmove.
   Context `{!dimsumGS Σ} `{!recGS Σ}.
 
-  Local Canonical Structure spec_mod_lang_unit.
-
   Let m_t := rec_link_trans {["main"; "memmove"; "memcpy"]} {["locle"]} rec_trans (spec_trans rec_event ()).
 
+(*
   Lemma memmove_sim :
     rec_state_interp (rec_init (main_prog ∪ memmove_prog ∪ memcpy_prog)) None -∗
     (MLFRun None, [], rec_init (main_prog ∪ memmove_prog ∪ memcpy_prog), (locle_spec, ())) ⪯{m_t,
@@ -1100,8 +1122,9 @@ Section memmove.
     iIntros "Hγσ_s Hγσ_t Hγκ".
     iApply "Hs". iSplit!.
   Qed.
+*)
 
-  Lemma memmove_sim2 :
+  Lemma memmove_sim :
     rec_state_interp (rec_init (main_prog ∪ memmove_prog ∪ memcpy_prog)) None -∗
     (MLFRun None, [], rec_init (main_prog ∪ memmove_prog ∪ memcpy_prog), (locle_spec, ())) ⪯{m_t,
       spec_trans rec_event ()} (main_spec, ()).
@@ -1113,26 +1136,30 @@ Section memmove.
     iMod (mstate_var_alloc (option rec_event)) as (γκ) "Hγκ".
     (* iMod (mstate_var_alloc (list seq_product_case)) as (γs) "Hγs". *)
     (* iMod (mstate_var_alloc (m_state (spec_trans rec_event ()))) as (γσ_locle) "Hγσ_locle". *)
+    iMod (mstate_var_alloc unit) as (γs) "?".
+    iMod (mstate_var_split γs tt with "[$]") as "[Hγs ?]".
     iModIntro.
+    pose (Hspec := SpecGS γs).
+
     iApply (sim_tgt_constP_intro γσ_t γσ_s γκ with "Hγσ_t Hγσ_s Hγκ [-]"). iIntros "Hγσ_s".
     iApply (sim_tgt_link_None with "[-]").
     iIntros "!>" (??????). destruct!/=. case_match; destruct!/=.
     iApply (sim_tgt_constP_elim γσ_t γσ_s γκ with "[Hγσ_s] [-]"); [done..|].
     iIntros "Hγσ_s Hγσ_t Hγκ".
-    iApply (sim_gen_expr_intro _ tt _ None with "[] [-]"); [simpl; done..|].
-    iApply (sim_gen_expr_wand _ _ _ _ _ (λ _, False%I) with "[-] []"); [|by iIntros].
+    iApply (sim_gen_expr_intro _ tt with "[Hγs] [-]"); [simpl; done..|].
     iEval (unfold main_spec). rewrite /TReceive bind_bind.
     iApply (sim_src_TExist (_, _, _)).
     rewrite bind_bind. setoid_rewrite bind_ret_l.
-    iApply sim_gen_TVis. iIntros ([]) "_".
+    iApply sim_gen_TVis. iIntros ([]) "Hγs". iIntros (??) "[-> [-> _]]".
     iApply (sim_src_constP_next with "[Hγσ_t] [Hγκ] [Hγσ_s] [%] [-]"); [done..|].
     iIntros "Hγσ_s". iApply sim_gen_stop.
     iApply (sim_tgt_constP_elim γσ_t γσ_s γκ with "[Hγσ_s] [-]"); [done..|].
     iIntros "Hγσ_s Hγσ_t Hγκ".
-    iApply (sim_gen_expr_intro _ tt _ None with "[] [-]"); [simpl; done..|].
+    iApply (sim_gen_expr_intro _ tt with "[Hγs] [-]"); [simpl; done..|].
     iApply sim_src_TAssume. iIntros (?).
     iApply sim_src_TAssume. iIntros (?). simplify_eq.
-    iApply sim_gen_expr_None => /=. iIntros (? [] ??) "_".
+    iApply sim_gen_expr_steps => /=. iIntros (? [] ?) "Hγs".
+    iApply (sim_gen_stop with "[-]"). iIntros (??) "[-> [-> _]]".
 
     rewrite bool_decide_true; [|done].
     iApply (sim_src_constP_next with "[Hγσ_t] [Hγκ] [Hγσ_s] [%] [-]"); [done..|].
@@ -1148,45 +1175,31 @@ Section memmove.
     iMod (rec_mapsto_alloc_big (h_heap h) with "Hh") as "[Hh _]". { apply map_disjoint_empty_r. }
     iModIntro.
 
-    iApply (sim_gen_expr_intro _ [] _ None with "[Hh Ha]"). { done. }
+    iApply (sim_gen_expr_intro _ [] with "[Hh Ha]"). { done. }
     { rewrite /= /rec_state_interp dom_empty_L right_id_L /=. iFrame "#∗". by iApply rec_alloc_fake. }
 
     set (Π := link_tgt_leftP _ _ _ _).
-    (* set (Π := directMH Tgt _). *)
-
-    have MHnop : inMH _ Tgt nopMH Π. {
-      unfold inMH. iIntros "!>" (???) "HΠ Hσ".
-      iDestruct "HΠ" as (->) "C" => /=.
-      iIntros (?) "Hγσ_s ??". iApply sim_gen_stop.
-      iIntros (??) "??".
-      iDestruct (mstate_var_merge with "[$] [$]") as (->) "Hγσ_t".
-      iDestruct (mstate_var_merge with "[$] [$]") as (->) "Hγκ".
-      iSplit!.
-      iApply (sim_tgt_constP_intro_weak with "[Hγσ_t] [Hγσ_s] [Hγκ] [-]"); [done..|].
-      iApply (sim_tgt_link_left with "[-]").
-      iApply (sim_gen_wand with "[C Hσ]"); [by iApply "Hσ"|].
-      iIntros (??) "HC". iApply ("HC").
-    }
 
     iApply (sim_gen_expr_bind _ [ReturnExtCtx _] with "[-]") => /=.
     iApply (sim_main_full with "[] [] [] [] [] Hγσ_s"). 1-4: by iApply (rec_fn_intro with "[$]").
     { iIntros "!>". iApply sim_locle2. 1: done. 1: { by iApply (rec_fn_intro with "[$]"). }
       iIntros (??). iDestruct 1 as (?? ->) "HC" => /=.
       iIntros (??????). destruct!/=. rewrite bool_decide_false //. rewrite bool_decide_true //.
-      iApply (sim_tgt_link_right_recv with "[-]"). iApply "HC". iIntros (??). iDestruct 1 as (? ->) "HC" => /=.
+      iApply (sim_tgt_link_right_recv with "[-]"). iApply "HC". iSplit!. iIntros (??). iDestruct 1 as (? ->) "HC" => /=.
       iIntros (?). simplify_eq.
-      iApply (sim_tgt_link_right with "[-]"). iApply "HC"; [done|].
+      iApply (sim_tgt_link_right with "[-]"). iApply "HC". iSplit!.
       iIntros (??). iDestruct 1 as (?? -> ->) "HC" => /=.
       iIntros (??????). destruct!/=.
-      iApply (sim_tgt_link_left_recv with "[-]"). iApply "HC". iIntros (??). iDestruct 1 as (? ->) "HC" => /=.
+      iApply (sim_tgt_link_left_recv with "[-]"). iApply "HC". iSplit!.
+      iIntros (??). iDestruct 1 as (? ->) "HC" => /=.
       iIntros (?). simplify_eq.
       iApply (sim_tgt_link_left with "[-]"). by iApply "HC". } { done. }
     iSplit!.
-    - unfold letstar. iIntros "!>" (??). iDestruct 1 as (??? ->) "[Hγσ_s HC]" => /=.
+    - iIntros "!>" (??). iDestruct 1 as (??? ->) "[Hγσ_s HC]" => /=.
       iIntros  (??????). destruct!/=. rewrite !bool_decide_false //.
       iApply (sim_tgt_constP_elim γσ_t γσ_s γκ with "[Hγσ_s] [-]"); [done..|].
       iIntros "Hγσ_s Hγσ_t Hγκ".
-      iApply "HC". iIntros (??). iDestruct 1 as (->) "HC".
+      iApply "HC". iSplit!. iIntros (??). iDestruct 1 as (->) "HC".
       iApply (sim_src_constP_next with "[Hγσ_t] [Hγκ] [Hγσ_s] [%] [-]"); [done..|].
       iIntros "Hγσ_s".
       iApply (sim_tgt_link_None with "[-]"). iIntros "!>" (??????). destruct!/=.
@@ -1197,16 +1210,18 @@ Section memmove.
       iIntros "Hγσ_s". iApply sim_gen_stop.
       iApply (sim_tgt_constP_elim γσ_t γσ_s γκ with "[Hγσ_s] [-]"); [done..|].
       iIntros "Hγσ_s Hγσ_t Hγκ".
-      iApply "HC". iIntros (??). iDestruct 1 as (?? -> ->) "HC".
+      iApply "HC". iSplit!. iIntros (??). iDestruct 1 as (?? -> ->) "HC".
       iApply (sim_src_constP_next with "[Hγσ_t] [Hγκ] [Hγσ_s] [%] [-]"); [done..|].
       iIntros "Hγσ_s". destruct!/=.
       iApply (sim_tgt_link_left_recv with "[-]").
-      iApply ("HC" with "[-]"). iFrame. iIntros (??). iDestruct 1 as (? ->) "HC".
+      iApply ("HC" with "[-]"). iFrame. iSplit!.
+      iIntros (??). iDestruct 1 as (? ->) "HC".
       iIntros (?). simplify_eq.
       iApply (sim_tgt_link_left with "[-]").
       iApply "HC". iSplit!.
-    - iIntros (?) "Hγσ_s Hs". iApply sim_tgt_rec_ReturnExt. iIntros (???) "Hfns''' Hh Ha !>".
-      iIntros "?" => /=. iIntros (??????). destruct!/=.
+    - iIntros (?) "[% [Hγσ_s [Hs %]]]". iApply sim_tgt_rec_ReturnExt.
+      iIntros (???) "Hfns''' Hh Ha !>".
+      iIntros (??) "[-> [-> _]]" => /=. iIntros (??????). destruct!/=.
       iApply (sim_tgt_constP_elim γσ_t γσ_s γκ with "[Hγσ_s] [-]"); [done..|].
       iIntros "Hγσ_s Hγσ_t Hγκ".
       iApply "Hs".
